Added files for memory interpolation lemmas, and suitably adapted compiler_correctness_trans.
mem_interpolants.v: defines a module type with all four lemmas using
   CompCert's standard notions. compiler_correctness_trans now assumes
   a module of this type.
mem_interpolation_defs.v: collects various useful lemmas and constructions,
   Also contains almost all modifications that we require of CompCert's
   memory model, currently in the form of Axioms claiming their
   (of course not really satisfied) equivalence to the official versions.
mem_interpolation_EE.v / mem_interpolation_EI.v / 
mem_interpolation_IE.v / mem_interpolation_II.v: the proofs of the four
  lemmas (cases extend-extend, extend-inject, inject-extend and   
  inject-inject). In addition to the axioms from mem_interpolation_defs.v,
  these files only contain axioms asserting the existence of Mem.content/
   Mem.access maps, for the appropriately characterizations of these maps.
   These axioms thus amount to a form of constructiveness of memories.
mem_interpolation_proofs.v: combines the four lemmas to an implementation of the module type from mem_interpolants.v

compositional_compcert/mem_lemmas.v
@@ -248,133 +248,427 @@ Proof. intros. intros  b Hb.
   split; eauto. 
 Qed. 
 
-(** * A value that is (if its a pointer) not dangling wrt m - a condition
-like this will probably be need to imposed on after-external return
-values (and thus also on the values returned by safely-halted)*)
+Lemma compose_meminjD_Some: forall j jj b b2 ofs2, 
+       (compose_meminj j jj) b = Some(b2,ofs2) -> 
+       exists b1, exists ofs1, exists ofs,
+       j b = Some(b1,ofs1) /\ jj b1 = Some(b2,ofs) /\ ofs2=ofs1+ofs. 
+Proof. unfold compose_meminj; intros.
+       remember (j b) as z; destruct z; apply eq_sym in Heqz.
+         destruct p. exists b0. exists z. 
+         remember (jj b0) as zz. 
+         destruct zz; apply eq_sym in Heqzz. 
+           destruct p. inv H. exists z0. auto.
+           inv H.
+         inv H.
+Qed. 
 
+Lemma compose_meminj_inject_incr: forall j12 j12' j23 j23'
+  (InjIncr12: inject_incr j12 j12') (InjIncr23: inject_incr j23 j23'),
+  inject_incr (compose_meminj j12 j23) (compose_meminj j12' j23').
+Proof.
+  intros. intros b; intros. 
+  apply compose_meminjD_Some in H. 
+  destruct H as [b1 [ofs1 [ofs [Hb [Hb1 Hdelta]]]]]. 
+  unfold compose_meminj.
+  rewrite (InjIncr12 _ _ _ Hb).
+  rewrite (InjIncr23 _ _ _ Hb1). subst. trivial.
+Qed.
+
+Lemma compose_meminj_inject_separated: forall j12 j12' j23 j23' m1 m2 m3
+   (InjSep12 : inject_separated j12 j12' m1 m2)
+   (InjSep23 : inject_separated j23 j23' m2 m3)
+   (InjIncr12: inject_incr j12 j12') (InjIncr23: inject_incr j23 j23')
+   (BV12: forall b1 b2 ofs, j12 b1 = Some (b2,ofs) -> Mem.valid_block m1 b1 /\ Mem.valid_block m2 b2)
+   (BV23: forall b1 b2 ofs, j23 b1 = Some (b2,ofs) -> Mem.valid_block m2 b1 /\ Mem.valid_block m3 b2),
+   inject_separated (compose_meminj j12 j23) (compose_meminj j12' j23') m1 m3.
+Proof. intros.
+  unfold compose_meminj; intros b; intros.
+  remember (j12 b) as j12b.
+  destruct j12b; inv H; apply eq_sym in Heqj12b. destruct p.
+    rewrite (InjIncr12 _ _ _ Heqj12b) in H0.
+    remember (j23 b0) as j23b0.
+    destruct j23b0; inv H2; apply eq_sym in Heqj23b0. destruct p. inv H1.
+    remember (j23' b0) as j23'b0.
+    destruct j23'b0; inv H0; apply eq_sym in Heqj23'b0. destruct p. inv H1.
+    destruct (InjSep23 _ _ _ Heqj23b0 Heqj23'b0).    
+    split; trivial. exfalso. apply H. eapply BV12. apply Heqj12b.
+  remember (j12' b) as j12'b.
+  destruct j12'b; inv H0; apply eq_sym in Heqj12'b. destruct p.
+    destruct (InjSep12 _ _ _ Heqj12b Heqj12'b). split; trivial.
+    remember (j23' b0) as j23'b0.
+    destruct j23'b0; inv H1; apply eq_sym in Heqj23'b0. destruct p. inv H3.
+    remember (j23 b0) as j23b0.
+    destruct j23b0; apply eq_sym in Heqj23b0. destruct p. rewrite (InjIncr23 _ _ _ Heqj23b0) in Heqj23'b0. inv Heqj23'b0.      
+      exfalso. apply H0. eapply BV23. apply Heqj23b0.
+    destruct (InjSep23 _ _ _ Heqj23b0 Heqj23'b0). assumption.    
+Qed.
+
+Lemma compose_meminj_inject_separated': forall j12 j12' j23 j23' m1 m2 m3
+   (InjSep12 : inject_separated j12 j12' m1 m2)
+   (InjSep23 : inject_separated j23 j23' m2 m3)
+   (InjIncr12: inject_incr j12 j12') (InjIncr23: inject_incr j23 j23')
+   (MInj12: Mem.inject j12 m1 m2)
+   (MInj23: Mem.inject j23 m2 m3),
+   inject_separated (compose_meminj j12 j23) (compose_meminj j12' j23') m1 m3.
+Proof. intros.
+  eapply compose_meminj_inject_separated; try eassumption.
+  intros; split. apply (Mem.valid_block_inject_1 _ _ _ _ _ _ H MInj12). apply (Mem.valid_block_inject_2 _ _ _ _ _ _ H MInj12).
+  intros; split. apply (Mem.valid_block_inject_1 _ _ _ _ _ _ H MInj23). apply (Mem.valid_block_inject_2 _ _ _ _ _ _ H MInj23).
+Qed.
+
+Lemma forall_lessdef_refl: forall vals,  Forall2 Val.lessdef vals vals.
+Proof. induction vals; econstructor; trivial. Qed.
+
+Lemma lessdef_hastype: forall v v' (V:Val.lessdef v v') T, Val.has_type v' T -> Val.has_type v T.
+Proof. intros. inv V; simpl; trivial. Qed.
+
+Lemma forall_lessdef_hastype: forall vals vals' (V:Forall2 Val.lessdef vals vals') Ts 
+          (HTs: Forall2 Val.has_type vals' Ts), Forall2 Val.has_type vals Ts.
+Proof.
+  intros vals vals' V.
+  induction V; simpl in *; intros.
+       trivial.
+  inv HTs. constructor. eapply  lessdef_hastype; eassumption. apply (IHV _ H4).
+Qed.
+
+Lemma valinject_hastype:  forall j v v' (V: (val_inject j) v v') T, Val.has_type v' T -> Val.has_type v T.
+Proof. intros. inv V; simpl; trivial. Qed.
+
+Lemma forall_valinject_hastype:  forall j vals vals' (V:  Forall2 (val_inject j) vals vals') 
+                Ts (HTs: Forall2 Val.has_type vals' Ts), Forall2 Val.has_type vals Ts.
+Proof.
+  intros j vals vals' V.
+  induction V; simpl in *; intros.
+       trivial.
+  inv HTs. constructor. eapply  valinject_hastype; eassumption. apply (IHV _ H4).
+Qed.
+
+Lemma val_inject_split: forall v1 v3 j12 j23 (V: val_inject (compose_meminj j12 j23) v1 v3),
+             exists v2, val_inject j12 v1 v2 /\ val_inject j23 v2 v3. 
+Proof. intros. 
+   inv V. 
+     exists (Vint i). split; constructor.
+     exists (Vfloat f). split; constructor. 
+     apply compose_meminjD_Some in H. rename b2 into b3.
+       destruct H as [b2 [ofs2 [ofs3 [J12 [J23 DD]]]]]; subst. 
+       eexists. split. econstructor. apply J12. reflexivity. 
+          econstructor. apply J23. rewrite Int.add_assoc.
+          assert (H: Int.repr (ofs2 + ofs3) = Int.add (Int.repr ofs2) (Int.repr ofs3)). 
+            clear - ofs2 ofs3. rewrite Int.add_unsigned.
+            apply Int.eqm_samerepr. apply Int.eqm_add; apply Int.eqm_unsigned_repr.
+          rewrite H. trivial. 
+     exists Vundef. split; constructor.
+Qed.     
+
+Lemma forall_lessdef_trans: forall vals1 vals2 (V12: Forall2 Val.lessdef vals1 vals2) 
+                                                               vals3  (V23: Forall2 Val.lessdef vals2 vals3) ,  Forall2 Val.lessdef vals1 vals3.
+Proof. intros vals1 vals2 V12. 
+   induction V12; intros; inv V23; econstructor.
+   eapply Val.lessdef_trans; eauto.
+          eapply IHV12; trivial.
+Qed.
+
+Lemma extends_loc_out_of_bounds: forall m1 m2 (Ext: Mem.extends m1 m2) b ofs,
+                loc_out_of_bounds m2 b ofs -> loc_out_of_bounds m1 b ofs.
+Proof. intros.
+  inv Ext. inv mext_inj.
+  intros N.  eapply H. apply (mi_perm _ b 0) in N. rewrite Zplus_0_r in N. assumption. reflexivity.
+Qed.
+
+Lemma extends_loc_out_of_reach: forall m1 m2 (Ext: Mem.extends m1 m2) b ofs j
+               (Hj: loc_out_of_reach j m2 b ofs), loc_out_of_reach j m1 b ofs.
+Proof. intros. unfold loc_out_of_reach in *. intros.
+           intros N. eapply (Hj _ _ H). clear Hj H. inv Ext. inv mext_inj.
+           specialize (mi_perm b0 _ 0 (ofs - delta) Max Nonempty (eq_refl _)). rewrite Zplus_0_r in mi_perm. apply (mi_perm N).
+Qed.
+
+Lemma valinject_lessdef: forall v1 v2 v3 j (V12:val_inject j v1 v2) (V23 : Val.lessdef v2 v3),val_inject j v1 v3.
+Proof. intros. 
+   inv V12; inv V23; try constructor.
+    econstructor. eassumption. trivial.
+Qed.
+
+Lemma forall_valinject_lessdef: forall vals1 vals2 j (VInj12 : Forall2 (val_inject j) vals1 vals2) vals3 
+                  (LD23 : Forall2 Val.lessdef vals2 vals3), Forall2 (val_inject j) vals1 vals3.
+Proof. intros vals1 vals2 j VInj12.
+   induction VInj12; intros; inv LD23. constructor.
+     econstructor. eapply valinject_lessdef; eassumption.
+          eapply (IHVInj12 _ H4).
+Qed.
+
+Lemma val_lessdef_inject_compose: forall v1 v2 (LD12 : Val.lessdef v1 v2) j v3
+              (InjV23 : val_inject j v2 v3), val_inject j v1 v3.
+Proof. intros. 
+  apply val_inject_id in LD12.
+  apply (val_inject_compose _ _ _ _ _ LD12) in InjV23.
+  rewrite compose_idL in InjV23. assumption.
+Qed. 
+
+Lemma forall_val_lessdef_inject_compose: forall v1 v2 (LD12 : Forall2 Val.lessdef v1 v2) j v3
+              (InjV23 : Forall2 (val_inject j) v2 v3), Forall2 (val_inject j) v1 v3.
+Proof. intros v1 v2 H.
+  induction H; intros; inv InjV23; econstructor.
+       eapply val_lessdef_inject_compose; eassumption.
+       apply (IHForall2 _ _ H5). 
+Qed. 
+
+Lemma forall_val_inject_compose: forall vals1 vals2 j1 (ValsInj12 : Forall2 (val_inject j1) vals1 vals2)
+                vals3 j2 (ValsInj23 : Forall2 (val_inject j2) vals2 vals3),
+              Forall2 (val_inject (compose_meminj j1 j2)) vals1 vals3.
+Proof.
+  intros vals1 vals2 j1 ValsInj12.
+  induction ValsInj12; intros; inv ValsInj23; econstructor.
+     eapply val_inject_compose; eassumption.
+  apply (IHValsInj12 _ _ H4).
+Qed.
+
+Lemma val_inject_flat: forall m1 m2 j (Inj: Mem.inject j m1 m2) v1 v2 (V: val_inject j v1 v2),
+                val_inject  (Mem.flat_inj (Mem.nextblock m1)) v1 v1.
+Proof. intros.
+  inv V; try constructor.
+    apply val_inject_ptr with (delta:=0).
+            unfold Mem.flat_inj. inv Inj.
+            remember (zlt b1 (Mem.nextblock m1)).
+            destruct s. trivial. assert (j b1 = None). apply mi_freeblocks. apply z. rewrite H in H0. inv H0.
+            rewrite Int.add_zero. trivial.
+Qed.
+
+Lemma forall_val_inject_flat: forall m1 m2 j (Inj: Mem.inject j m1 m2) vals1 vals2
+                (V: Forall2 (val_inject j) vals1 vals2),
+                Forall2 (val_inject  (Mem.flat_inj (Mem.nextblock m1))) vals1 vals1.
+Proof. intros.
+  induction V; intros; try econstructor.
+       eapply val_inject_flat; eassumption.
+  apply IHV.
+Qed.
+
+Lemma po_trans: forall a b c, Mem.perm_order'' a b ->  Mem.perm_order'' b c ->
+      Mem.perm_order'' a c.
+Proof. intros.
+   destruct a; destruct b; destruct c; simpl in *; try contradiction; try trivial.
+   eapply perm_order_trans; eassumption.
+Qed.
+
+Lemma extends_perm: forall m1 m2 (Ext: Mem.extends m1 m2) b ofs k p,
+   Mem.perm m1 b ofs k p -> Mem.perm m2 b ofs k p.  
+Proof. intros. destruct Ext. destruct mext_inj.
+  specialize (mi_perm b b 0 ofs k p (eq_refl _) H).
+  rewrite Zplus_0_r in mi_perm. assumption.
+Qed.
+
+Lemma extends_permorder: forall m1 m2 (Ext: Mem.extends m1 m2) b ofs k,
+  Mem.perm_order'' (ZMap.get b (Mem.mem_access m2) ofs k)
+                   (ZMap.get b (Mem.mem_access m1) ofs k).
+Proof.
+  intros. destruct Ext.  destruct mext_inj as [prm _ _].
+  specialize (prm b b 0 ofs k). unfold Mem.perm in prm. 
+  remember ((ZMap.get b (Mem.mem_access m2) ofs k)) as z.
+  destruct z; apply eq_sym in Heqz; simpl  in *. 
+    remember ((ZMap.get b (Mem.mem_access m1) ofs k)) as zz.
+    destruct zz; trivial; apply eq_sym in Heqzz; simpl  in *.
+       rewrite Zplus_0_r in prm. rewrite Heqz in prm. 
+       specialize (prm p0 (eq_refl _)). apply prm. apply perm_refl. 
+  remember ((ZMap.get b (Mem.mem_access m1) ofs k)) as zz.
+    destruct zz; trivial; apply eq_sym in Heqzz; simpl  in *.
+       rewrite Zplus_0_r in prm. rewrite Heqz in prm. 
+       specialize (prm p (eq_refl _)). exfalso. apply prm. apply perm_refl. 
+Qed.
+
+Lemma fwd_maxperm: forall m1 m2 (FWD: mem_forward m1 m2) b 
+  (V:Mem.valid_block m1 b) ofs p,
+  Mem.perm m2 b ofs Max p -> Mem.perm m1 b ofs Max p.
+Proof. intros. apply FWD; assumption. Qed. 
+
+Lemma fwd_maxpermorder: forall m1 m2 (FWD: mem_forward m1 m2) b 
+  (V:Mem.valid_block m1 b) ofs,
+  Mem.perm_order'' (ZMap.get b (Mem.mem_access m1) ofs Max)
+                   (ZMap.get b (Mem.mem_access m2) ofs Max).
+Proof.
+  intros. destruct (FWD b); try assumption. 
+  remember ((ZMap.get b (Mem.mem_access m2) ofs Max)) as z.
+  destruct z; apply eq_sym in Heqz; simpl  in *.
+  remember ((ZMap.get b (Mem.mem_access m1) ofs Max)) as zz.
+  destruct zz; apply eq_sym in Heqzz; simpl  in *.
+  specialize (H0 ofs p).  unfold Mem.perm in H0. unfold Mem.perm_order' in H0. 
+  rewrite Heqz in H0. rewrite Heqzz in H0. apply H0. apply perm_refl.
+  specialize (H0 ofs p).  unfold Mem.perm in H0. unfold Mem.perm_order' in H0. 
+  rewrite Heqz in H0. rewrite Heqzz in H0. apply H0. apply perm_refl.
+
+
+  remember ((ZMap.get b (Mem.mem_access m1) ofs Max)) as zz.
+  destruct zz; apply eq_sym in Heqzz; simpl in *; trivial.
+Qed.
+
+Lemma po_oo: forall p q, Mem.perm_order' p q = Mem.perm_order'' p (Some q).
+Proof. intros. destruct p; trivial. Qed. 
+
+Lemma inject_permorder: forall j m1 m2 (Inj : Mem.inject j m1 m2) b b' ofs'
+      (J: j b = Some (b', ofs')) ofs k,
+     Mem.perm_order'' (ZMap.get b' (Mem.mem_access m2) (ofs + ofs') k)
+     (ZMap.get b (Mem.mem_access m1) ofs k).
+Proof.
+  intros. destruct Inj. destruct mi_inj as [prm _ _ ].
+  specialize (prm b b' ofs' ofs k). unfold Mem.perm in prm. 
+  remember ((ZMap.get b' (Mem.mem_access m2) (ofs + ofs') k)) as z.
+  destruct z; apply eq_sym in Heqz; simpl  in *. 
+    remember ((ZMap.get b (Mem.mem_access m1) ofs k)) as zz.
+    destruct zz; trivial; apply eq_sym in Heqzz; simpl  in *.
+       eapply prm. apply J. apply perm_refl. 
+  remember ((ZMap.get b (Mem.mem_access m1) ofs k)) as zz.
+    destruct zz; trivial; apply eq_sym in Heqzz; simpl  in *.
+       eapply prm. apply J. apply perm_refl. 
+Qed.
+
+Lemma PermExtNotnonempty: forall m1 m2 (Inj: Mem.extends m1 m2) b ofs p
+     (H: ~ Mem.perm m2 b ofs p Nonempty),  ~ Mem.perm m1 b ofs p Nonempty.
+Proof. intros. destruct Inj. destruct mext_inj.
+intros N. apply H. apply (mi_perm _ _ _ _ _ _ (eq_refl _)) in N. rewrite Zplus_0_r in N. apply N.
+Qed.
+
+Lemma  PermInjNotnonempty: forall j m1 m2 (Inj: Mem.inject j m1 m2) b b2 delta (J:j b = Some(b2,delta)) ofs p
+     (H:  ~ Mem.perm m2 b2 (ofs+delta) p Nonempty), ~ Mem.perm m1 b ofs p Nonempty.
+Proof. intros. destruct Inj. destruct mi_inj.
+intros N. apply H. apply (mi_perm _ _ _ _ _ _ J) in N. apply N.
+Qed.
+
+Lemma mem_unchanged_on_refl: forall m f, mem_unchanged_on f m m.
+Proof. intros. split; intros; trivial. Qed.
+
+Lemma inject_LOOR_LOOB: forall m1 m2 j (Minj12 : Mem.inject j m1 m2) m3 m3', 
+  mem_unchanged_on (loc_out_of_reach j m1) m3 m3' -> 
+  mem_unchanged_on (loc_out_of_bounds m2) m3 m3'.
+Proof. intros.
+     split; intros; eapply H; trivial.
+         intros b2; intros. unfold loc_out_of_bounds in H0. intros N. apply H0.
+                          inv Minj12. inv mi_inj. apply (mi_perm _ _ _ _ _ _ H2) in N.
+                         rewrite <- Zplus_comm in N. rewrite Zplus_minus in N.  apply N.
+    intros. apply H0 in H2.
+         intros b2; intros. unfold loc_out_of_bounds in H2. intros N. apply H2.
+                          inv Minj12. inv mi_inj. apply (mi_perm _ _ _ _ _ _ H3) in N.
+                         rewrite <- Zplus_comm in N. rewrite Zplus_minus in N.  apply N.
+Qed.
+
+(*A value that is (if its a pointer) not dangling wrt m - a condition
+ like this will probably be need to imposed on after-external return
+ values (and thus also on the values returned by safely-halted)*)
 Definition val_valid (v:val) (m:mem):Prop := 
-  match v with Vptr b ofs => Mem.valid_block m b | _ => True end.
+     match v with Vptr b ofs => Mem.valid_block m b | _ => True 
+     end.
 
-(** In fact, valid vals is a slight relaxtion of valid pointers*)
-
+(*In fact val_valid is a slight relaxtion of valid_pointer*)
 Lemma valid_ptr_val_valid: forall b ofs m, 
-  Mem.valid_pointer m b ofs = true -> val_valid (Vptr b (Int.repr ofs)) m.
+    Mem.valid_pointer m b ofs = true -> val_valid (Vptr b (Int.repr ofs)) m.
 Proof. intros.
   apply Mem.valid_pointer_nonempty_perm in H. eapply Mem.perm_valid_block. apply H.
 Qed.
 
-(** * Memories that do not contain "dangling pointers"*)
+Lemma extends_valvalid: forall m1 m2 (Ext: Mem.extends m1 m2) v,
+        val_valid v m1 <-> val_valid v m2.
+Proof. intros.
+  split; intros. destruct v; simpl in *; try econstructor.
+     eapply (Mem.valid_block_extends _ _ _ Ext). apply H. 
+  destruct v; simpl in *; try econstructor.
+     eapply (Mem.valid_block_extends _ _ _ Ext). apply H.
+Qed.
 
+Lemma inject_valvalid: forall j m1 m2 (Inj: Mem.inject j m1 m2) v2 (V:val_valid v2 m2) v1,
+             val_inject j v1 v2 -> val_valid v1 m1.
+Proof. intros.
+  inv H. constructor. constructor.
+     simpl in *. eapply Mem.valid_block_inject_1; eassumption. 
+     constructor. 
+Qed. 
+
+(*memories that do not contain "dangling pointers"*)
 Definition mem_wd m := Mem.inject_neutral (Mem.nextblock m) m.
 
 Lemma mem_wdI: forall m,
-  (forall b ofs  (R:Mem.perm m b ofs Cur Readable),
-    memval_inject  (Mem.flat_inj (Mem.nextblock m)) 
-    (ZMap.get ofs (ZMap.get b (Mem.mem_contents m)))
-    (ZMap.get ofs (ZMap.get b (Mem.mem_contents m)))) -> mem_wd m.
+    (forall b ofs  (R:Mem.perm m b ofs Cur Readable),
+                memval_inject  (Mem.flat_inj (Mem.nextblock m)) 
+                                             (ZMap.get ofs (ZMap.get b (Mem.mem_contents m)))
+                                            (ZMap.get ofs (ZMap.get b (Mem.mem_contents m)))) -> mem_wd m.
 Proof. intros.
   split; intros.
-  apply flatinj_E in  H0. destruct H0 as [? [? ?]]; subst. rewrite Zplus_0_r. 
-   trivial. 
-  apply flatinj_E in  H0. destruct H0 as [? [? ?]]; subst. rewrite Zplus_0_r. 
-   trivial. 
-  apply flatinj_E in  H0. destruct H0 as [? [? ?]]; subst. rewrite Zplus_0_r.
-  apply H. apply H1.
+     apply flatinj_E in  H0. destruct H0 as [? [? ?]]; subst. rewrite Zplus_0_r. trivial. 
+     apply flatinj_E in  H0. destruct H0 as [? [? ?]]; subst. rewrite Zplus_0_r. trivial. 
+     apply flatinj_E in  H0. destruct H0 as [? [? ?]]; subst. rewrite Zplus_0_r.
+        apply H. apply H1.
 Qed.
-
-Lemma mem_wd_E: forall m, mem_wd m -> 
-  Mem.inject (Mem.flat_inj (Mem.nextblock m)) m m.
+        
+Lemma mem_wd_E: forall m, mem_wd m ->  Mem.inject (Mem.flat_inj (Mem.nextblock m)) m m.
 Proof. intros. apply Mem.neutral_inject. apply H. Qed.
 
 Lemma meminj_split_flatinjR: forall j m m' (J:Mem.inject j m' m), mem_wd m -> 
-  j = compose_meminj j (Mem.flat_inj (Mem.nextblock m)).
+     j = compose_meminj j (Mem.flat_inj (Mem.nextblock m)).
 Proof. intros. apply mem_wd_E in H.
-  unfold  compose_meminj.
-  apply extensionality. intro b. 
-  remember (j b). 
-  destruct o; trivial. destruct p. unfold Mem.flat_inj in *.
-  remember (zlt b0 (Mem.nextblock m)).
+   unfold  compose_meminj.
+   apply extensionality. intro b. 
+   remember (j b). 
+   destruct o; trivial. destruct p. unfold Mem.flat_inj in *.
+   remember (zlt b0 (Mem.nextblock m)).
   destruct s.  rewrite Zplus_0_r. trivial.
   inv J. apply eq_sym in Heqo. specialize (mi_mappedblocks _ _ _ Heqo).
-  exfalso. unfold Mem.valid_block in mi_mappedblocks. omega.
+               exfalso. unfold Mem.valid_block in mi_mappedblocks. omega.
 Qed.
 
 Lemma meminj_split_flatinjL: forall j m m' (J:Mem.inject j m m'), mem_wd m -> 
-  j = compose_meminj (Mem.flat_inj (Mem.nextblock m)) j.
+     j = compose_meminj (Mem.flat_inj (Mem.nextblock m)) j.
 Proof. intros. apply mem_wd_E in H.
-  unfold  compose_meminj.
-  apply extensionality. intro b. 
-  unfold Mem.flat_inj in *.
-  remember (zlt b (Mem.nextblock m)).
-  destruct s. remember (j b). destruct o. destruct p.  rewrite Zplus_0_l. trivial. 
-   trivial.
+   unfold  compose_meminj.
+   apply extensionality. intro b. 
+   unfold Mem.flat_inj in *.
+   remember (zlt b (Mem.nextblock m)).
+  destruct s. remember (j b). destruct o. destruct p.  rewrite Zplus_0_l. trivial. trivial.
   inv J. apply mi_freeblocks. apply z.
 Qed.
 
-(** Preservation of mem_wd by memory operations *)
-
+(*Preservation of mem_wd by memory operations*)
 Lemma mem_wd_empty: mem_wd Mem.empty.
-Proof. apply Mem.empty_inject_neutral. Qed.
+Proof.  apply Mem.empty_inject_neutral. Qed.
 
 Lemma  mem_wd_alloc: forall m b lo hi m' (ALL: Mem.alloc m lo hi = (m',b))
-  (WDm: mem_wd m), mem_wd m'.
+     (WDm: mem_wd m), mem_wd m'.
 Proof. intros. unfold mem_wd in *.
   rewrite (Mem.nextblock_alloc _ _ _ _ _ ALL).
   eapply (Mem.alloc_inject_neutral _ _ _ _ _ _ ALL); try omega.
   inv WDm. 
-  split; intros. 
-  apply flatinj_E in H. destruct H as [? [? ?]]; subst. rewrite Zplus_0_r. 
-   assumption.
-  apply flatinj_E in H. destruct H as [? [? ?]]; subst. rewrite Zplus_0_r. 
-   assumption.
-  apply flatinj_E in H. destruct H as [? [? ?]]; subst. rewrite Zplus_0_r.
-  assert (X: Mem.flat_inj (Mem.nextblock m) b1 = Some (b1, 0)).
-  apply flatinj_I. apply (Mem.perm_valid_block _ _ _ _ _ H0).
-  specialize (mi_memval _ _ _ _ X H0). rewrite Zplus_0_r in mi_memval.
-  eapply memval_inject_incr; try eassumption.
-  intros bb; intros. eapply flatinj_mono; try eassumption. omega.
+         split; intros. 
+             apply flatinj_E in H. destruct H as [? [? ?]]; subst. rewrite Zplus_0_r. assumption.
+             apply flatinj_E in H. destruct H as [? [? ?]]; subst. rewrite Zplus_0_r. assumption.
+             apply flatinj_E in H. destruct H as [? [? ?]]; subst. rewrite Zplus_0_r.
+                 assert (X: Mem.flat_inj (Mem.nextblock m) b1 = Some (b1, 0)).
+                     apply flatinj_I. apply (Mem.perm_valid_block _ _ _ _ _ H0).
+                  specialize (mi_memval _ _ _ _ X H0). rewrite Zplus_0_r in mi_memval.
+                  eapply memval_inject_incr; try eassumption.
+                       intros bb; intros. eapply flatinj_mono; try eassumption. omega.
 Qed. 
 
 Lemma  mem_wd_drop: forall m b lo hi p m' (DROP: Mem.drop_perm m b lo hi p = Some m')
-  (WDm: mem_wd m), Mem.valid_block m b -> mem_wd m'.
+     (WDm: mem_wd m), Mem.valid_block m b -> mem_wd m'.
 Proof. intros. unfold mem_wd in *.
   rewrite (Mem.nextblock_drop _ _ _ _ _ _ DROP).
   eapply (Mem.drop_inject_neutral _ _ _ _ _ _ _ DROP); trivial.
 Qed.
-
+  
 Lemma free_neutral: forall (thr : block) (m : mem) (lo hi : Z) (b : block) (m' : Mem.mem')
   (FREE: Mem.free m b lo hi = Some m'),
   Mem.inject_neutral thr m -> Mem.inject_neutral thr m'.
 Proof. intros. inv H. 
   split; intros.
-  apply flatinj_E in H. destruct H as [? [? ?]]; subst. rewrite Zplus_0_r. 
-   assumption.
-  apply flatinj_E in H. destruct H as [? [? ?]]; subst. rewrite Zplus_0_r. 
-   assumption.
-  apply flatinj_E in H. destruct H as [? [? ?]]; subst. rewrite Zplus_0_r.
-  assert (X: Mem.flat_inj thr b1 = Some (b1,0)). apply flatinj_I. 
-   assumption.
-  assert (Y:= Mem.perm_free_3 _ _ _ _ _ FREE _ _ _ _ H0).
-  specialize (mi_memval _ _ _ _ X Y). 
-  rewrite Zplus_0_r in *.
-  assert (Heq: ZMap.get ofs (ZMap.get b1 (Mem.mem_contents m))=
-               ZMap.get ofs (ZMap.get b1 (Mem.mem_contents m'))).
-   Transparent Mem.free. (*Maybe there's a an appropriate lemma in Memory.v, but 
-                            I couldn't find it.*)
-   unfold Mem.free in FREE.
-   destruct (Mem.range_perm_dec m b lo hi Cur Freeable); try solve[congruence].
-   solve[inv FREE; unfold Mem.unchecked_free; simpl; auto].
-  destruct (ZMap.get ofs (ZMap.get b1 (Mem.mem_contents m'))); 
-   try constructor.
-  destruct (ZMap.get ofs (ZMap.get b1 (Mem.mem_contents m))); 
-    congruence.
+     apply flatinj_E in H. destruct H as [? [? ?]]; subst. rewrite Zplus_0_r. assumption.
+     apply flatinj_E in H. destruct H as [? [? ?]]; subst. rewrite Zplus_0_r. assumption.
+     apply flatinj_E in H. destruct H as [? [? ?]]; subst. rewrite Zplus_0_r.
+        assert (X: Mem.flat_inj thr b1 = Some (b1,0)). apply flatinj_I. assumption.
+        assert (Y:= Mem.perm_free_3 _ _ _ _ _ FREE _ _ _ _ H0).
+         specialize (mi_memval _ _ _ _ X Y). rewrite Zplus_0_r in *.    
+         rewrite (Mem.free_result _ _ _ _ _ FREE) in *. simpl in *. apply mi_memval.
 Qed.
 
 Lemma mem_wd_free: forall m b lo hi m' (WDm: mem_wd m)
   (FREE: Mem.free m b lo hi = Some m'), mem_wd m'.
 Proof. intros. unfold mem_wd in *.
   eapply free_neutral. apply FREE.
-  rewrite (Mem.nextblock_free _ _ _ _ _ FREE). assumption.
+   rewrite (Mem.nextblock_free _ _ _ _ _ FREE). assumption.
 Qed.
 
 Lemma mem_wd_store: forall m b ofs v m' chunk (WDm: mem_wd m)
@@ -382,13 +676,32 @@ Lemma mem_wd_store: forall m b ofs v m' chunk (WDm: mem_wd m)
   (V: val_valid v m), mem_wd m'.
 Proof. intros. unfold mem_wd in *.
   eapply Mem.store_inject_neutral. apply ST.
-  rewrite (Mem.nextblock_store _ _ _ _ _ _ ST). assumption.
-  assert (X:= Mem.store_valid_access_3 _ _ _ _ _ _ ST).
-  rewrite (Mem.nextblock_store _ _ _ _ _ _ ST). 
-  apply (Mem.valid_access_implies _ _ _ _ _  Nonempty) in X.
-  apply Mem.valid_access_valid_block in X. apply X.
-  constructor.
-  rewrite (Mem.nextblock_store _ _ _ _ _ _ ST). 
-  destruct v. constructor. constructor. constructor. 
-  econstructor. eapply flatinj_I. apply V. rewrite Int.add_zero. trivial.
+      rewrite (Mem.nextblock_store _ _ _ _ _ _ ST). assumption.
+      assert (X:= Mem.store_valid_access_3 _ _ _ _ _ _ ST).
+          rewrite (Mem.nextblock_store _ _ _ _ _ _ ST). 
+           apply (Mem.valid_access_implies _ _ _ _ _  Nonempty) in X.
+                apply Mem.valid_access_valid_block in X. apply X.
+            constructor.
+      rewrite (Mem.nextblock_store _ _ _ _ _ _ ST). 
+          destruct v. constructor. constructor. constructor.  econstructor. eapply flatinj_I. apply V. rewrite Int.add_zero. trivial.
 Qed.
+
+Lemma extends_memwd: forall m1 m2 (Ext: Mem.extends m1 m2), mem_wd m2 -> mem_wd m1.
+Proof.
+  intros. eapply mem_wdI. intros.
+  assert (Mem.perm m2 b ofs Cur Readable).
+    eapply (Mem.perm_extends _ _ _ _ _ _ Ext R).
+  assert (Mem.valid_block m2 b).
+     apply (Mem.perm_valid_block _ _ _ _ _ H0). 
+  destruct Ext. rewrite mext_next.
+  assert (Mem.flat_inj (Mem.nextblock m2) b = Some (b,0)).
+    apply flatinj_I. apply H1.
+  destruct mext_inj. specialize (mi_memval b ofs b 0 (eq_refl _) R). rewrite Zplus_0_r in mi_memval.
+  destruct H. specialize (mi_memval0 b ofs b 0 H2 H0). rewrite Zplus_0_r in mi_memval0. 
+  remember (ZMap.get ofs (ZMap.get b (Mem.mem_contents m1))) as v.
+  destruct v. constructor. constructor.
+    econstructor. eapply flatinj_I. inv mi_memval. inv H4. rewrite Int.add_zero in H6. 
+      rewrite <- H6 in mi_memval0. simpl in mi_memval0. inversion mi_memval0.
+      apply flatinj_E in H4. apply H4. 
+   rewrite Int.add_zero. reflexivity.
+Qed. 
