compositional_compcert/mem_interpolation_II.v
@@ -1,0 +1,2178 @@
+Load loadpath.
+Require Import Events. (*is needed for some definitions (loc_unmapped etc, and
+  also at the very end of this file, in order to convert between the 
+  tweaked and the standard definitions of mem_unchanged_on etc, and for
+  being able to remove/add inject_permorder/extends_permorder etc*)
+Require Import Memory.
+Require Import Coqlib.
+Require Import Integers.
+Require Import Values.
+Require Import Maps.
+
+Require Import compositional_compcert.mem_lemmas.
+Require Import compositional_compcert.mem_interpolation_defs.
+
+Fixpoint mkInjectionsN (N:nat)(n1 n2:block)(j k l: meminj) 
+                     :  meminj * meminj * Z * Z:= 
+   match N with O => (j,k,n1,n2)
+    | S M => mkInjectionsN M (n1+1) (n2 + 1)
+                             (fun b => if eq_block b n1 
+                                       then Some (n2,0) 
+                                       else j b)
+                             (fun b => if eq_block b n2 then l n1 else k b)
+                             l
+   end.
+
+Lemma mkInjectionsN_0: forall N n1 n2 j k l j' k' n1' n2'
+    (HI: mkInjectionsN N n1 n2 j k l = (j',k',n1',n2')),
+    n1 + Z_of_nat N = n1' /\ n2 + Z_of_nat N = n2'.
+Proof. intros N.
+  induction N; simpl; intros. 
+     inv HI. repeat rewrite Zplus_0_r. split; trivial.
+     specialize (IHN _ _ _ _ _ _ _ _ _ HI). clear HI.
+     rewrite Zpos_P_of_succ_nat. omega.
+Qed.
+
+Lemma mkInjectionsN_1: forall N n1 n2 j k l j' k' n1' n2'
+    (HI: mkInjectionsN N n1 n2 j k l = (j',k',n1',n2')),
+    forall b1 b2 ofs2 (Jb: j b1 = Some(b2,ofs2)), 
+    b1 < n1 -> j' b1 = Some (b2,ofs2).
+Proof. intros N.
+  induction N; simpl; intros. 
+     inv HI. apply Jb.
+     specialize (IHN _ _ _ _ _ _ _ _ _ HI). clear HI.
+        apply (IHN b1 b2 ofs2). clear IHN.
+        remember (eq_block b1 n1) as d.
+        destruct d; clear Heqd. exfalso. subst. clear -H. omega.
+        assumption.
+     omega.
+Qed.
+
+Lemma mkInjectionsN_2: forall N n1 n2 j k l j' k' n1' n2'
+    (HI: mkInjectionsN N n1 n2 j k l = (j',k',n1',n2')),
+    forall b2 b3 ofs3 (Jb: k b2 = Some(b3,ofs3)), 
+    b2 < n2 -> k' b2 = Some (b3,ofs3).
+Proof. intros N.
+  induction N; simpl; intros. 
+     inv HI. apply Jb.
+     specialize (IHN _ _ _ _ _ _ _ _ _ HI). clear HI.
+        apply (IHN b2 b3 ofs3). clear IHN.
+        remember (eq_block b2 n2) as d.
+        destruct d; clear Heqd. exfalso. subst. clear -H. omega.
+        assumption.
+      omega.
+Qed.
+
+Lemma mkInjectionsN_3: forall N n1 n2 j k l j' k' n1' n2'
+        (HI: mkInjectionsN N n1 n2 j k l = (j',k',n1',n2')) b1 b2 ofs2,
+        j' b1 = Some(b2,ofs2) -> 
+     (j b1 = Some (b2,ofs2)) \/ 
+     (exists m, 0 <= m /\ b1 = n1 + m /\ b2=n2 + m /\ ofs2=0).
+Proof. intros N.
+  induction N; simpl; intros. 
+      inv HI. left. trivial.
+  specialize (IHN _ _ _ _ _ _ _ _ _ HI _ _ _ H).  clear HI H.
+  destruct IHN.  
+      remember (eq_block b1 n1) as d.
+      destruct d; clear Heqd. inv H. right. exists Z0. 
+      repeat rewrite Zplus_0_r. split. omega. auto.
+      left; trivial.
+ destruct H as [m [? [? [? ?]]]]. right. subst. 
+   exists (1+m). unfold block in *. omega.
+Qed.
+
+Lemma mkInjectionsN_3V: forall N n1 n2 j k l j' k' n1' n2'
+     (HI: mkInjectionsN N n1 n2 j k l = (j',k',n1',n2')) 
+     (HJ: forall b1 b2 ofs2, j b1 = Some(b2,ofs2) -> b1 < n1 /\ b2 < n2)
+     (HK: forall b2 b3 ofs3, k b2 = Some(b3,ofs3) -> b2 < n2)
+     b1 b2 ofs2,
+     j' b1 = Some(b2,ofs2) -> 
+          (j b1 = Some (b2,ofs2) /\ b1 < n1 /\ b2 < n2) \/ 
+          (exists m, 0 <= m /\ b1 = n1 + m /\ b2=n2 + m /\ 
+                     ofs2=0 /\ b1 < n1' /\ b2<n2').
+Proof. intros N.
+  induction N; simpl; intros. 
+      inv HI. left. split; trivial. eapply HJ. apply H.
+  specialize (IHN _ _ _ _ _ _ _ _ _ HI).
+  assert (HJ': forall (b1 b2 : block) (ofs2 : Z),
+          (fun b : block => if eq_block b n1 then Some (n2, 0) else j b) b1 =
+            Some (b2, ofs2) 
+          -> b1 < n1 + 1 /\ b2 < n2 + 1). 
+      clear IHN. intros.
+      destruct (eq_block b0 n1); subst. inv H0. omega. 
+      specialize (HJ _ _ _ H0). omega.
+  assert (HK': forall (b2 b3 : block) (ofs3 : Z),
+       (fun b : block => if eq_block b n2 then l n1 else k b) b2 =
+           Some (b3, ofs3)
+       -> b2 < n2 + 1).
+     clear IHN. intros.
+     destruct (eq_block b0 n2); subst. omega. 
+     specialize (HK _ _ _ H0). omega.
+  specialize (IHN HJ' HK' _ _ _ H).  
+  apply mkInjectionsN_0 in HI.
+  destruct IHN.  
+     remember (eq_block b1 n1) as d.
+     destruct d; clear Heqd. subst. destruct H0 as [? [? ?]]. inv H0. right.
+           exists Z0. repeat rewrite Zplus_0_r. 
+           repeat (split; (try omega ; try auto)).
+     destruct H0 as [? [? ?]]. left. split. trivial.  apply HJ in H0. trivial.
+  destruct H0 as [m [? [? [? ?]]]]. right. subst. 
+    exists (1+m). unfold block in *. omega.
+Qed.
+
+Lemma mkInjectionsN_4: forall N n1 n2 j k l j' k' n1' n2' 
+       (HI: mkInjectionsN N n1 n2 j k l = (j',k',n1',n2')) b2 b3 ofs3,
+       k' b2 = Some(b3,ofs3) -> 
+                k b2 = Some (b3,ofs3) \/
+                (exists m, 0 <= m /\ b2 = n2 + m /\ l (n1+m) = Some(b3,ofs3)).
+Proof. intros N. 
+  induction N; simpl. intros. 
+     inv HI. left; trivial.
+  intros.
+  specialize (IHN (n1+1) (n2+1) _ _ _ _ _ _ _ HI _ _ _ H).  clear HI H.
+  destruct IHN.  
+     remember (eq_block b2 n2) as d.
+     destruct d; clear Heqd. 
+          subst. right. exists Z0. repeat rewrite Zplus_0_r. 
+          split. omega. auto.
+     left; trivial.
+  destruct H as [m [? [? ?]]]. subst. 
+    right. exists (1+m). unfold block in *. 
+      split. omega.
+      split. omega. 
+      assert (n1 + (1 + m) = n1 + 1 + m). omega. 
+      rewrite H0. trivial.
+Qed.
+
+Lemma mkInjectionsN_4Val: forall N n1 n2 j k l j' k' n1' n2' 
+       (HI: mkInjectionsN N n1 n2 j k l = (j',k',n1',n2')) 
+       (HK: forall b2 b3 ofs3, k b2 = Some(b3,ofs3) -> b2 < n2) b2 b3 ofs3,
+       k' b2 = Some(b3,ofs3) -> 
+            (k b2 = Some (b3,ofs3) /\ b2 < n2) \/
+            (exists m, 0 <= m /\ b2 = n2 + m /\ 
+                       l (n1+m) = Some(b3,ofs3) /\ b2 < n2').
+Proof. intros N. 
+  induction N; simpl. intros. 
+     inv HI. left. split. trivial. apply HK in H. trivial.
+  intros.
+  assert (HK': (forall (b2 b3 : block) (ofs3 : Z),
+           (fun b : block => if eq_block b n2 then l n1 else k b) b2 =
+           Some (b3, ofs3) -> b2 < n2 + 1)). 
+      clear IHN HI. intros.
+      destruct (eq_block b0 n2); subst. omega. apply HK in H0. omega.
+  specialize (IHN _ _ _ _ _ _ _ _ _ HI HK' _ _ _ H).  
+  apply mkInjectionsN_0 in HI.
+  destruct IHN.  
+     remember (eq_block b2 n2) as d.
+     destruct d; clear Heqd. destruct H0. subst.
+          right. exists Z0. repeat rewrite Zplus_0_r. 
+          repeat (split ; (try omega ; try auto)).
+     destruct H0. left. split. trivial. omega.
+  destruct H0 as [m [? [? ?]]]. subst.  right.
+  exists (1+m). unfold block in *. 
+    split. omega.
+    split. omega. 
+    assert (n1 + (1 + m) = n1 + 1 + m). omega. 
+    rewrite H1. trivial.
+Qed.
+
+Lemma mkInjectionsN_5: forall N n1 n2 j k l j' k' n1' n2'
+       (HI: mkInjectionsN N n1 n2 j k l = (j',k',n1',n2')) 
+       (HJ1: forall b1 b2 ofs2, j b1 = Some(b2,ofs2) -> b1 < n1)
+       (HJ2: forall b1 b2 ofs2, j b1 = Some(b2,ofs2) ->b2 < n2)
+       (HK: forall b2 b3 ofs3, k b2 = Some(b3,ofs3) -> b2 < n2)
+       (HL: forall b1 b3 ofs3, l b1 = Some(b3,ofs3) -> b1 < n1')
+       b2 (HB: b2 < n2'),
+       k' b2 = None -> 
+             (b2 < n2 /\ k b2 = None) \/
+             (exists m, 0<=m /\ b2 = n2+m /\  l (n1+m) = None).
+Proof. intros N. 
+  induction N; simpl. intros. 
+     inv HI. left. split; trivial.
+  intros.
+  assert (HJ1': forall (b1 b2 : block) (ofs2 : Z),
+          (fun b : block => if eq_block b n1 then Some (n2, 0) else j b) b1 =
+          Some (b2, ofs2) -> b1 < n1 + 1).
+     clear IHN. intros.
+     destruct (eq_block b1 n1); subst. inv H0. omega. 
+     specialize (HJ1 _ _ _ H0). omega.
+  assert (HJ2': forall (b1 b2 : block) (ofs2 : Z),
+          (fun b : block => if eq_block b n1 then Some (n2, 0) else j b) b1 =
+           Some (b2, ofs2) -> b2 < n2 + 1). 
+     clear IHN. intros.
+     destruct (eq_block b1 n1); subst. inv H0. omega. 
+     specialize (HJ2 _ _ _ H0). omega.
+  assert (HK': forall (b2 b3 : block) (ofs3 : Z),
+          (fun b : block => if eq_block b n2 then l n1 else k b) b2 =
+          Some (b3, ofs3) -> b2 < n2 + 1).
+     clear IHN. intros.
+     destruct (eq_block b0 n2); subst. omega. 
+     specialize (HK _ _ _ H0). omega.
+  destruct (IHN _ _ _ _ _ _ _ _ _ HI HJ1' HJ2' HK' HL _ HB H).
+     destruct H0.
+     remember (eq_block b2 n2) as d.
+     destruct d; clear Heqd.
+          subst. right. exists Z0. repeat rewrite Zplus_0_r.
+              repeat (split; trivial). omega.
+     left. split; trivial. omega.
+  destruct H0 as [m [ HM [HBB HLL]]]. subst.
+    right. exists (1 + m). 
+    split. omega. 
+    assert (n1 + (1 + m) = n1 + 1 + m). omega. 
+    rewrite H0. split. omega. trivial.
+Qed.
+
+Lemma mkInjectionsN_6: forall N n1 n2 j k l j' k' n1' n2'
+    (HI: mkInjectionsN N n1 n2 j k l = (j',k',n1',n2')) b (J': j' b = None), 
+     j b = None.
+Proof. intros N.
+  induction N; simpl; intros. 
+     inv HI. trivial.
+     specialize (IHN _ _ _ _ _ _ _ _ _ HI _ J'). clear HI. simpl in IHN.
+     destruct (eq_block b n1); subst. inv IHN. trivial.
+Qed.
+
+Lemma mkInjectionsN_7: forall N n1 n2 j k l j' k' n1' n2'
+    (HI: mkInjectionsN N n1 n2 j k l = (j',k',n1',n2'))
+    b (HB: b < n1'),
+    (n1 <= b -> j' b  <> None) /\ (b < n1 -> j' b = j b).
+Proof. intros N.
+  induction N; intros; simpl.
+      intros. inv HI. split; intros.  exfalso. omega. trivial.
+  intros.
+     specialize (IHN _ _ _ _ _ _ _ _ _ HI _ HB). clear HI.
+     destruct IHN.
+     split; intros. 
+       apply Z_le_lt_eq_dec in H1. 
+       destruct H1. apply H. omega.
+       subst. remember (eq_block b b) as d. destruct d; clear Heqd. 
+              assert (b < b + 1). omega.
+              rewrite (H0 H1). intros Q. discriminate.
+         exfalso. apply n. trivial.
+   remember (eq_block b n1) as d.
+     destruct d; clear Heqd. subst. exfalso. omega.
+     apply H0. omega.
+Qed.
+
+Lemma mkInjectionsN_8: forall j' k' l n1' n2'  M N j  k n1 n2
+    (HI: mkInjectionsN N n1 n2 j k l = (j',k',n1',n2'))
+    (Hj: forall b, j b = None -> b < M \/ n1' <= b) b,
+    j' b = None -> b < M \/ n1' <= b. 
+Proof. intros j' k' l n1' n2' M N.
+  induction N; simpl; intros. 
+     inv HI. apply (Hj _ H).
+  specialize (IHN _ _ _ _ HI). clear HI.
+  apply IHN. intros.
+     remember (eq_block b0 n1) as d.
+    destruct d; clear Heqd; subst. inv H0.
+     apply Hj. apply H0.
+  apply H.
+Qed.
+
+Lemma mkInjectionsN_9: forall M j' k' l n1' n2'  N j  k n1 n2
+    (HI: mkInjectionsN N n1 n2 j k l = (j',k',n1',n2'))
+    (Hj: forall b, j b = None -> b < n1' -> b < M) b,
+    j' b = None -> b < n1' -> b < M.
+Proof. intros M j' k' l n1' n2' N.
+  induction N; simpl; intros. 
+     inv HI. apply (Hj _ H H0).
+  specialize (IHN _ _ _ _ HI). clear HI.
+  apply IHN. intros.
+     remember (eq_block b0 n1) as d.
+     destruct d; clear Heqd; subst. inv H1.
+       apply Hj. apply H1.
+    apply H2.
+ apply H.
+apply H0.
+Qed.
+
+Lemma mkInjectionsN_10: forall N n1 n2 j k l j' k' n1' n2'
+    (HI: mkInjectionsN N n1 n2 j k l = (j',k',n1',n2'))
+    (HL: forall b1 b3 ofs3, l b1 = Some(b3,ofs3) -> b1 < n1' - Z_of_nat N)
+    b b2 ofs2,
+    l b = Some(b2,ofs2) -> j' b = Some(b2,ofs2) \/ b < n1  + Z_of_nat N.
+Proof. intros N.
+  induction N; simpl; intros. 
+     inv HI. specialize (HL _ _ _ H). 
+     repeat rewrite Zminus_0_r in HL. rewrite Zplus_0_r. right; trivial.
+  assert (HN: forall (b1 b3 : block) (ofs3 : Z),
+       l b1 = Some (b3, ofs3) -> b1 < n1' - Z_of_nat N). 
+     intros. specialize (HL _ _ _ H0). rewrite Zpos_P_of_succ_nat in HL. omega. 
+ specialize (IHN _ _ _ _ _ _ _ _ _ HI HN _ _ _ H). clear HI.
+ destruct IHN.
+    left; trivial. 
+    rewrite Zpos_P_of_succ_nat. right. omega.
+Qed.
+
+Definition mkInjections (m1 m1' m2:mem) (j k l: meminj)
+                     :  meminj * meminj * Z * Z:= 
+  mkInjectionsN (nat_of_Z ((Mem.nextblock m1') - (Mem.nextblock m1)))
+                (Mem.nextblock m1)
+                (Mem.nextblock m2) j k l.
+
+Lemma mkInjections_1_injinc: forall m1 m1' m2 j k l j' k' n1' n2' 
+    (HI: mkInjections m1 m1' m2 j k l = (j',k',n1',n2'))
+    (VB: forall b1 b2 ofs2, j b1 = Some(b2,ofs2) -> Mem.valid_block m1 b1),
+    inject_incr j j'.
+Proof. unfold inject_incr, mkInjections; intros.
+   apply (mkInjectionsN_1 _ _ _ _ _ _ _ _ _ _ HI). apply H. eapply VB. apply H.
+Qed.
+
+Lemma mkInjections_1_injsep: forall m1 m1' m2 j k l j' k' n1' n2' 
+    (HI: mkInjections m1 m1' m2 j k l = (j',k',n1',n2')),
+    inject_separated j j' m1 m2.
+Proof. unfold inject_separated, mkInjections; intros.
+       specialize (mkInjectionsN_3 _ _ _ _ _ _ _ _ _ _ HI _ _ _ H0). intros.
+       destruct H1. rewrite H1 in H. discriminate.
+       destruct H1 as [m [? [? [? ?]]]]. subst.
+       clear HI H H0. unfold Mem.valid_block. omega.
+Qed.
+
+Lemma mkInjections_2_injinc: forall m1 m1' m2 j k l j' k' n1' n2' 
+        (HI: mkInjections m1 m1' m2 j k l = (j',k',n1',n2')) 
+        (VB: forall b1 b2 ofs2, k b1 = Some(b2,ofs2) -> Mem.valid_block m2 b1),
+      inject_incr k k'.
+Proof. 
+  unfold inject_incr, mkInjections; intros.
+  apply (mkInjectionsN_2 _ _ _ _ _ _ _ _ _ _ HI). apply H. eapply VB. apply H.
+Qed.
+
+Lemma mkInjections_2_injsep: forall m1 m1' m2 j k l j' k' n1' n2' 
+        (HI: mkInjections m1 m1' m2 j k l = (j',k',n1',n2'))
+        (VB: forall b1 b2 ofs2, j b1 = Some(b2,ofs2) -> Mem.valid_block m1 b1)
+         m3 (Sep:inject_separated (compose_meminj j k) l m1 m3),
+       inject_separated k k' m2 m3.
+Proof. 
+  unfold inject_separated, mkInjections; intros.
+  specialize (mkInjectionsN_4 _ _ _ _ _ _ _ _ _ _ HI _ _ _ H0). intros.
+  destruct H1. rewrite H1 in H. discriminate.
+  destruct H1 as [m [? [? ?]]]. subst. 
+  split. unfold Mem.valid_block. omega.
+  eapply (Sep (Mem.nextblock m1 + m)).
+     assert (HJ: j (Mem.nextblock m1 + m) = None).
+           remember (j (Mem.nextblock m1 + m)) as d. destruct d; trivial.
+           apply eq_sym in Heqd. destruct p. specialize (VB _ _ _ Heqd).
+           exfalso. clear - H1 VB. unfold Mem.valid_block in VB. omega.
+     unfold compose_meminj. rewrite HJ. trivial.
+  apply H3.
+Qed.
+
+Lemma mkInjections_6: forall m1 m1' m2 j k l j' k' n1' n2' 
+    (HI: mkInjections m1 m1' m2 j k l = (j',k',n1',n2')) b (J': j' b = None),
+     j b = None.
+Proof. intros. apply (mkInjectionsN_6 _ _ _ _ _ _ _ _ _ _ HI _ J'). Qed.
+
+Lemma mkInjections_5: forall m1 m1' m2 j k l j' k' n1' n2' 
+        (HI: mkInjections m1 m1' m2 j k l = (j',k',n1',n2'))
+        (VBj1: forall b1 b2 ofs2, j b1 = Some(b2,ofs2) -> Mem.valid_block m1 b1)
+        (VBj2: forall b1 b2 ofs2, j b1 = Some(b2,ofs2) -> Mem.valid_block m2 b2)
+        (VBk2: forall b1 b2 ofs2, k b1 = Some(b2,ofs2) -> Mem.valid_block m2 b1)
+        (VBl1: forall b1 b2 ofs2, l b1 = Some(b2,ofs2) -> b1 < n1')
+        b2 (HB: b2 < n2'),
+        k' b2 = None -> 
+        (Mem.valid_block m2 b2 /\ k b2 = None) \/
+        (exists m, 0<=m /\ b2 = Mem.nextblock m2 + m /\ 
+                   l (Mem.nextblock m1+m) = None).
+Proof. intros. unfold mkInjections in HI.
+  apply  (mkInjectionsN_5 _ _ _ _ _ _ _ _ _ _ HI VBj1 VBj2 VBk2 VBl1 _ HB H).
+Qed.
+
+Lemma J12'_no_overlap: forall m1 m2 j12 
+        (MInj12 : Mem.inject j12 m1 m2) m1' (Fwd1: mem_forward m1 m1') j23 m3
+        (MInj23 : Mem.inject j23 m2 m3) j' j12' j23' n1' n2'
+        (HeqMKI: mkInjections m1 m1' m2 j12 j23 j' = (j12', j23',n1',n2')),
+      Mem.meminj_no_overlap j12' m1'.
+Proof. intros. intros b b'; intros.
+  assert (Val1: (forall (b1 b2 : block) (ofs2 : Z),
+        j12 b1 = Some (b2, ofs2) ->
+        b1 < Mem.nextblock m1 /\ b2 < Mem.nextblock m2)).
+    intros; split.
+       eapply Mem.valid_block_inject_1. apply H4. eassumption.
+       eapply Mem.valid_block_inject_2. apply H4. eassumption.
+  assert (Val2: (forall (b2 b3 : block) (ofs3 : Z),
+        j23 b2 = Some (b3, ofs3) -> b2 < Mem.nextblock m2)).
+    intros.
+       eapply Mem.valid_block_inject_1. apply H4. eassumption.
+  assert (ZZ:= mkInjectionsN_3V  _ _ _ _ _ _ _ _ _ _ HeqMKI Val1 Val2 _ _ _ H0).
+  assert (ZZ':= mkInjectionsN_3V  _ _ _ _ _ _ _ _ _ _ 
+                HeqMKI Val1 Val2 _ _ _ H1).
+  destruct ZZ; destruct ZZ'.
+  (*j - j*) destruct H4 as [J [valJ1 valJ2]].
+            destruct H5 as [J' [valJ1' valJ2']].
+            eapply MInj12. apply H. assumption. assumption.
+                eapply Fwd1. apply valJ1. assumption.
+                eapply Fwd1. apply valJ1'. assumption.
+  (*j - fresh*) destruct H4 as [J [valJ1 valJ2]].
+                destruct H5 as [M [ZM [valJ1' [valJ2' [DD [leq1 leq2]]]]]].
+                subst.
+                left. intros ZZ; subst. omega.
+  (*fresh - j*) destruct H4 as [M [ZM [valJ1 [valJ2 [DD [leq1 leq2]]]]]].
+                subst.
+                destruct H5 as [J [valJ1' valJ2']].
+                left. intros ZZ; subst. omega.
+  (*fresh - fresh*)
+          destruct H4 as [M [ZM [valJ1 [valJ2 [DD [leq1 leq2]]]]]].
+          subst.
+          destruct H5 as [M' [ZM' [valJ1' [valJ2' [DD' [leq1' leq2']]]]]].
+          subst.
+          left. intros ZZ.
+          assert( M = M'). eapply Zplus_reg_l. apply ZZ.
+          subst. apply H. trivial.
+Qed.
+
+Lemma mkInjections_composememinj: forall m1 m1' m2 j k l j' k' n1' n2' 
+        (HI: mkInjections m1 m1' m2 j k l = (j',k',n1',n2'))
+        (InjIncr: inject_incr (compose_meminj j k) l) m3
+        (InjSep: inject_separated (compose_meminj j k) l m1 m3)
+        (VBj1: forall b1 b2 ofs2, j b1 = Some(b2,ofs2) -> Mem.valid_block m1 b1)
+        (VBj2: forall b1 b2 ofs2, j b1 = Some(b2,ofs2) -> Mem.valid_block m2 b2)
+        (VBk2: forall b1 b2 ofs2, k b1 = Some(b2,ofs2) -> Mem.valid_block m2 b1)
+        (VBL1': forall b1 b3 ofs3, l b1 = Some (b3, ofs3) -> b1 < n1'),
+      l = compose_meminj j' k'.
+Proof. intros.
+  extensionality b. 
+  remember (compose_meminj j' k' b) as z. 
+  destruct z; apply eq_sym in Heqz.
+     destruct p. apply  compose_meminjD_Some in Heqz. 
+     destruct Heqz as [b1 [ofs1 [ofs [J' [K' ZZ]]]]]. subst. 
+     unfold mkInjections in HI.
+     destruct (mkInjectionsN_3 _ _ _ _ _ _ _ _ _ _ HI _ _ _ J').
+         destruct (mkInjectionsN_4 _ _ _ _ _ _ _ _ _ _ HI _ _ _ K').
+            apply InjIncr. unfold compose_meminj. rewrite H. 
+                           rewrite H0. reflexivity.
+         destruct H0 as [m [NonNeg [B2 _]]]. subst. 
+              exfalso. specialize (VBj2 _ _ _ H).
+              clear - NonNeg VBj2. unfold Mem.valid_block in VBj2. omega.
+     destruct H as [m [NonNeg [B1 [B2 XX]]]]. subst.
+         destruct (mkInjectionsN_4 _ _ _ _ _ _ _ _ _ _ HI _ _ _ K'). 
+         exfalso. specialize (VBk2 _ _ _ H).
+         clear - NonNeg VBk2. unfold Mem.valid_block in VBk2. omega.
+     destruct H as [m' [NonNeg' [B2 ZZ]]].
+            assert (m=m'). clear - B2 NonNeg' NonNeg. 
+               apply Zplus_minus_eq in B2. subst. omega. 
+            subst. apply ZZ.
+  remember (l b) as lb. 
+  destruct lb; trivial. 
+  apply eq_sym in Heqlb. destruct p as [b2 ofs2]. 
+  unfold compose_meminj in Heqz.
+  remember (j' b) as j'b.
+  destruct j'b; apply eq_sym in Heqj'b.
+  (*J' b = Some*)
+      destruct p.
+      assert (K'None: k' b0 = None).
+          remember (k' b0) as kb.
+          destruct kb; apply eq_sym in Heqkb; inv Heqz; trivial. 
+             destruct p. inv H0.
+          rewrite K'None in Heqz. clear Heqz.
+      assert (KNone:k b0 = None).
+          remember (k b0) as d. destruct d; trivial. 
+             apply eq_sym in Heqd. destruct p.
+             apply (mkInjections_2_injinc _ _ _ _ _ _ _ _ _ _ HI VBk2) in Heqd. 
+             rewrite Heqd in K'None. discriminate.
+      assert (VBj : forall b1 b3 ofs3, j b1 = Some (b3, ofs3) -> 
+                     b1 < Mem.nextblock m1 /\ b3 < Mem.nextblock m2).
+             intros. split. eapply VBj1. apply H.  eapply VBj2. apply H.
+      destruct (mkInjectionsN_3V _ _ _ _ _ _ _ _ _ _ HI VBj VBk2 _ _ _ Heqj'b).
+      (*j b = Some*) destruct H as [? [? ?]].
+           assert (JKNone: compose_meminj j k b = None).
+               unfold compose_meminj. rewrite H. rewrite KNone. reflexivity.
+           destruct (InjSep _ _ _ JKNone Heqlb). exfalso. apply (H2 H0).
+      (*other case*) 
+           destruct H as [m [Nonneg [B1 [B2 [? [? ?]]]]]]; subst.
+           destruct (mkInjections_5 _ _ _ _ _ _ _ _ _ _ HI VBj1 
+                       VBj2 VBk2 VBL1' _ H1 K'None).
+           (*case 1 valid in m2 - contradiction*)
+               destruct H as [XX _]. clear -XX Nonneg. 
+               unfold Mem.valid_block in XX. exfalso. omega.
+           (*case 2 - l undefined - contradiction*)
+                         destruct H as [mm [MMnoneg [MM LL]]].
+                         assert (mm= m). clear - MM. omega. subst.
+                         rewrite LL in Heqlb. discriminate.
+     (*J' b = None*)
+           assert (Jb:= mkInjections_6  _ _ _ _ _ _ _ _ _ _ HI _ Heqj'b).
+           assert (CMN: compose_meminj j k b = None).
+                   unfold compose_meminj. rewrite Jb. trivial.
+           destruct (InjSep _ _ _ CMN Heqlb) as [NV1 _].
+           apply VBL1' in Heqlb. 
+           destruct (mkInjectionsN_7 _ _ _ _ _ _ _ _ _ _ HI _ Heqlb) as [X _].
+           rewrite Heqj'b in X. exfalso.
+           apply X. 
+              clear - NV1. unfold Mem.valid_block in NV1. omega.
+              trivial.
+Qed. 
+
+Definition removeUndefs (j l j':meminj):meminj := 
+   fun b => match j b with 
+              None => match l b with 
+                         None => None | Some (b1,delta1) => j' b 
+                      end
+            | Some(b2,delta2) => Some(b2, delta2)
+            end.
+
+Lemma RU_composememinj: forall m1 m1' m2 j k l j' k' n1' n2' 
+       (HI: mkInjections m1 m1' m2 j k l = (j',k',n1',n2'))
+       (InjIncr: inject_incr (compose_meminj j k) l) m3
+       (InjSep: inject_separated (compose_meminj j k) l m1 m3)
+       (VBj1: forall b1 b2 ofs2, j b1 = Some(b2,ofs2) -> Mem.valid_block m1 b1)
+       (VBj2: forall b1 b2 ofs2, j b1 = Some(b2,ofs2) -> Mem.valid_block m2 b2)
+       (VBk2: forall b1 b2 ofs2, k b1 = Some(b2,ofs2) -> Mem.valid_block m2 b1)
+       (VBL1': forall b1 b3 ofs3, l b1 = Some (b3, ofs3) -> b1 < n1'),
+      l = compose_meminj (removeUndefs j l j') k'.
+Proof. intros.
+  assert (INC:= mkInjections_1_injinc _ _ _ _ _ _ _ _ _ _ HI VBj1). 
+  subst.
+  rewrite (mkInjections_composememinj _ _ _ _ _ _ _ _ _ _ HI InjIncr _ 
+                 InjSep VBj1 VBj2 VBk2 VBL1').
+  extensionality b. unfold removeUndefs. 
+  remember (compose_meminj j' k' b) as V.
+  destruct V; apply eq_sym in HeqV.
+    destruct p. unfold compose_meminj in *.
+      remember (j' b) as v1.
+      destruct v1; apply eq_sym in Heqv1; inv HeqV.
+        destruct p.
+        remember (k' b1) as v2.
+        destruct v2; apply eq_sym in Heqv2; inv H0.
+          destruct p. inv H1.
+          remember (j b) as v3. 
+          destruct v3; apply eq_sym in Heqv3.
+             destruct p. 
+             rewrite (INC _ _ _ Heqv3) in Heqv1. inv Heqv1. 
+             rewrite Heqv2.  trivial.
+         rewrite Heqv2. trivial.
+   unfold compose_meminj in *.
+      remember (j b) as v1.
+      destruct v1; apply eq_sym in Heqv1.
+          destruct p. apply INC in Heqv1. 
+                      rewrite Heqv1 in *. rewrite HeqV. trivial.
+      rewrite HeqV. trivial.
+Qed. 
+
+Lemma RU_D: forall j j' (I: inject_incr j j') l, 
+            inject_incr (removeUndefs j l j') j'.
+Proof. intros. intros b; intros.
+  unfold removeUndefs in H.
+  remember (j b) as d.
+  destruct d; apply eq_sym in Heqd.
+      destruct p. inv H. apply (I _ _ _  Heqd).
+  remember (l b) as d.
+  destruct d; apply eq_sym in Heqd; try inv H.
+      destruct p. trivial. 
+Qed.
+
+Lemma inc_RU: forall j j' (I: inject_incr j j') l, 
+              inject_incr j (removeUndefs j l j').
+Proof. intros. intros b; intros.
+  unfold removeUndefs. rewrite H. trivial.
+Qed.
+
+Lemma meminij_no_overlap_inject_incr: 
+   forall j m (NOV: Mem.meminj_no_overlap j m) k (K:inject_incr k j),
+  Mem.meminj_no_overlap k m.
+Proof. intros.
+  intros b; intros.
+  apply K in H0. apply K in H1.
+  eapply (NOV _ _ _ _ _ _ _ _  H H0 H1 H2 H3).
+Qed.
+
+Lemma RU_no_overlap: 
+     forall m1 m2 j12 (MInj12 : Mem.inject j12 m1 m2) m1'
+            (Fwd1: mem_forward m1 m1') j23 m3
+            (MInj23 : Mem.inject j23 m2 m3) j' j12' j23' n1' n2'
+            (HeqMKI: mkInjections m1 m1' m2 j12 j23 j' = (j12',j23',n1',n2')),
+            Mem.meminj_no_overlap (removeUndefs j12 j' j12') m1'.
+Proof. 
+intros.
+specialize (J12'_no_overlap _ _ _ MInj12 _ Fwd1 _ _ MInj23 _ _ _ _ _ HeqMKI). 
+intros.
+  eapply (meminij_no_overlap_inject_incr _ _ H).
+  apply RU_D.
+  eapply (mkInjections_1_injinc _ _ _ _ _ _ _ _ _ _ HeqMKI).
+  intros. apply (Mem.valid_block_inject_1 _ _ _ _ _ _ H0 MInj12).
+Qed.
+
+Definition inject_memval (j:meminj) (v:memval): memval := 
+     match v with 
+         Pointer b ofs n =>
+             match j b with 
+                None => Undef
+              | Some(b',delta) => Pointer b' (Int.add ofs (Int.repr delta)) n 
+             end
+       | _ => v
+     end.
+
+Lemma inject_memval_memval_inject: forall j v v' 
+  (IM: inject_memval j v = v') (U: v' <> Undef), memval_inject j v v'.
+Proof.
+  intros.
+  destruct v; destruct v'; simpl in *; try inv IM; try constructor. 
+     exfalso. apply U. trivial.
+     rewrite H0.
+        remember (j b) as d. destruct d. destruct p. inv H0. inv H0.
+     rewrite H0. 
+        remember (j b) as d.
+        destruct d. 
+          destruct p. inv H0.
+            eapply memval_inject_ptr. rewrite <- Heqd. reflexivity. 
+          trivial. 
+        inv H0.
+Qed.
+
+Lemma inject_memval_memval_inject1: forall j v 
+               (H: forall b ofs n, v = Pointer b ofs n -> 
+                                   exists p, j b = Some p),
+               memval_inject j v (inject_memval j v). 
+Proof.
+  intros.
+  destruct v; simpl in *; try constructor.
+  specialize (H _ _ _ (eq_refl _)). 
+  destruct H. rewrite H. destruct x. econstructor. apply H. trivial.
+Qed.
+
+Definition AccessMap_II_Property  (j12 j12' :meminj) (m1 m1' m2 : mem)
+           (AM:ZMap.t (Z -> perm_kind -> option permission)):Prop :=
+  forall b2, 
+    (Mem.valid_block m2 b2 -> forall k ofs2,
+         match source j12 m1 b2 ofs2 with
+             Some(b1,ofs1) =>  ZMap.get b2 AM ofs2 k = 
+                               ZMap.get b1 m1'.(Mem.mem_access) ofs1 k
+           | None =>  ZMap.get b2 AM ofs2 k = 
+                      ZMap.get b2 m2.(Mem.mem_access) ofs2 k
+           end)
+     /\ (~ Mem.valid_block m2 b2 -> forall k ofs2,
+           match source j12' m1' b2 ofs2 with 
+              Some(b1,ofs1) => ZMap.get b2 AM ofs2 k =
+                               ZMap.get b1 m1'.(Mem.mem_access) ofs1 k
+            | None =>  ZMap.get b2 AM ofs2 k = None
+          end).
+
+Definition Content_II_Property (j12 j12' j23':meminj) (m1 m1' m2:Mem.mem)
+                               (CM:ZMap.t (ZMap.t memval)):=
+  forall b2, 
+      (Mem.valid_block m2 b2 -> forall ofs2,
+         match source j12 m1 b2 ofs2 with
+             Some(b1,ofs1) =>
+                 match j23' b2 with
+                    None => ZMap.get ofs2 (ZMap.get b2 CM) =
+                            ZMap.get ofs2 (ZMap.get b2 m2.(Mem.mem_contents))
+                 | Some(b3,ofs3) => 
+                      ZMap.get ofs2 (ZMap.get b2 CM) = 
+                        inject_memval j12' 
+                            (ZMap.get ofs1 (ZMap.get b1 m1'.(Mem.mem_contents)))
+                 end
+           | None => ZMap.get ofs2 (ZMap.get b2 CM) =
+                     ZMap.get ofs2 (ZMap.get b2 m2.(Mem.mem_contents))
+         end)
+  /\ (~ Mem.valid_block m2 b2 -> forall ofs2,
+         match source j12' m1' b2 ofs2 with
+                None => ZMap.get ofs2 (ZMap.get b2 CM) =Undef
+              | Some(b1,ofs1) =>
+                   ZMap.get ofs2 (ZMap.get b2 CM) =
+                     inject_memval j12' 
+                       (ZMap.get ofs1 (ZMap.get b1 m1'.(Mem.mem_contents)))
+         end).
+
+(*
+Lemma mkInjections_aligned_1: forall m1 m1' m2 j k l j' k' n1' n2' 
+                   (HI: mkInjections m1 m1' m2 j k l = (j',k',n1',n2')) 
+                   (A: inject_aligned j), inject_aligned j'.
+Proof. intros. intros b; intros.
+  destruct (mkInjectionsN_3  _ _ _ _ _ _ _ _ _ _ HI _ _ _ H).
+        apply (A _ _ _ H0).
+  destruct H0 as [? [? [? [? ?]]]]. subst. 
+  split. omega. intros. apply Zdivide_0.
+Qed.
+
+Lemma mkInjections_aligned_2: forall m1 m1' m2 j k l j' k' n1' n2' 
+                 (HI: mkInjections m1 m1' m2 j k l = (j',k',n1',n2')) 
+                 (Ik: inject_aligned k) (Il: inject_aligned l), 
+                 inject_aligned k'.
+Proof. intros. intros b; intros.
+  destruct (mkInjectionsN_4  _ _ _ _ _ _ _ _ _ _ HI _ _ _ H).
+        apply (Ik _ _ _ H0).
+  destruct H0 as [? [? [? ?]]]. subst. 
+        apply (Il _ _ _ H2).
+Qed.*)
+
+Lemma mkInjections_aligned_1: forall m1 m1' m2 j k l j' k' n1' n2' 
+                       (HI: mkInjections m1 m1' m2 j k l = (j',k',n1',n2')) 
+                       (A: inject_aligned j), inject_aligned j'.
+Proof. intros. intros b; intros.
+  destruct (mkInjectionsN_3  _ _ _ _ _ _ _ _ _ _ HI _ _ _ H).
+     apply (A _ _  _ H0).
+  destruct H0 as [? [? [? [? ?]]]]. subst.  apply Zdivide_0.
+Qed.
+
+Lemma mkInjections_aligned_2: forall m1 m1' m2 j k l j' k' n1' n2' 
+                       (HI: mkInjections m1 m1' m2 j k l = (j',k',n1',n2')) 
+                       (Ik: inject_aligned k) (Il: inject_aligned l),
+                       inject_aligned k'.
+Proof. intros. intros b; intros.
+  destruct (mkInjectionsN_4  _ _ _ _ _ _ _ _ _ _ HI _ _ _ H).
+        apply (Ik _ _ _ H0).
+  destruct H0 as [? [? [? ?]]]. subst. 
+        apply (Il _ _ _ H2).
+Qed.
+
+Lemma II_ok: forall m1 m2 j12 (MInj12 : Mem.inject j12 m1 m2) m1'
+                   (Fwd1: mem_forward m1 m1') j23 m3
+                   (MInj23 : Mem.inject j23 m2 m3) m3'
+                   (Fwd3: mem_forward m3 m3')
+                   j' (MInj13': Mem.inject j' m1' m3')
+                   (InjIncr: inject_incr (compose_meminj j12 j23) j')
+                   (InjSep: inject_separated (compose_meminj j12 j23) j' m1 m3)
+                   (Unch11': my_mem_unchanged_on 
+                             (loc_unmapped (compose_meminj j12 j23)) m1 m1')
+                   (Unch33': my_mem_unchanged_on
+                         (loc_out_of_reach (compose_meminj j12 j23) m1) m3 m3')
+                   (WD1: mem_wd m1) (WD1': mem_wd m1') (WD2: mem_wd m2)
+                   (WD3: mem_wd m3) (WD3' : mem_wd m3')
+
+                   (IP12: inject_perm_nonempty j12 m1 m2)
+                   (IP23: inject_perm_nonempty j23 m2 m3)
+                   (IPj': inject_perm_nonempty j' m1' m3')
+
+                   prej12' j23' n1' n2'
+                   (HeqMKI: mkInjections m1 m1' m2 j12 j23 j' = 
+                            (prej12', j23', n1', n2'))
+                   j12' (Hj12': j12'= removeUndefs j12 j' prej12')
+                   m2'
+                   (NB: m2'.(Mem.nextblock)=n2')
+                   (CONT:  Content_II_Property j12 j12' j23' m1 m1' m2 
+                                               (m2'.(Mem.mem_contents)))
+                   (ACCESS: AccessMap_II_Property j12 j12' m1 m1' m2 
+                                                  (m2'.(Mem.mem_access)))
+                   (AL12: inject_aligned j12) (AL23: inject_aligned j23)
+                   (AL13': inject_aligned j'), 
+                j'=compose_meminj j12' j23' /\
+                     inject_aligned j12'  /\ inject_aligned j23' /\
+                     inject_incr j12 j12' /\ inject_incr j23 j23' /\
+                     Mem.inject j12' m1' m2' /\ mem_forward m2 m2' /\ 
+                     Mem.inject j23' m2' m3' /\
+                     my_mem_unchanged_on (loc_out_of_reach j12 m1) m2 m2' /\
+                     inject_separated j12 j12' m1 m2 /\
+                     inject_separated j23 j23' m2 m3 /\
+                     my_mem_unchanged_on (loc_unmapped j23) m2 m2' /\ 
+                     my_mem_unchanged_on (loc_out_of_reach j23 m2) m3 m3' /\
+                     (mem_wd m2 -> mem_wd m2') /\
+                     inject_perm_nonempty j12' m1' m2' /\
+                     inject_perm_nonempty j23' m2' m3'.
+Proof. intros.  
+  assert (VBj12_1: forall (b1 b2 : block) (ofs2 : Z),
+                   j12 b1 = Some (b2, ofs2) -> Mem.valid_block m1 b1).
+      intros. apply (Mem.valid_block_inject_1 _ _ _ _ _ _ H MInj12).
+  assert (VBj12_2: forall (b1 b2 : block) (ofs2 : Z),
+                   j12 b1 = Some (b2, ofs2) -> Mem.valid_block m2 b2).
+      intros. apply (Mem.valid_block_inject_2 _ _ _ _ _ _ H MInj12).
+  assert (VBj23_1: forall (b1 b2 : block) (ofs2 : Z),
+                   j23 b1 = Some (b2, ofs2) -> Mem.valid_block m2 b1).
+      intros. apply (Mem.valid_block_inject_1 _ _ _ _ _ _ H MInj23).
+  assert (VBj23_2: forall (b1 b2 : block) (ofs2 : Z),
+                   j23 b1 = Some (b2, ofs2) -> Mem.valid_block m3 b2).
+      intros. apply (Mem.valid_block_inject_2 _ _ _ _ _ _ H MInj23).
+  assert (VB12: forall (b3 b4 : block) (ofs3 : Z), 
+                 j12 b3 = Some (b4, ofs3) -> 
+                b3 < Mem.nextblock m1 /\ b4 < Mem.nextblock m2).
+      intros. split. apply (VBj12_1 _ _ _ H). apply (VBj12_2 _ _ _ H).
+  assert (preinc12:= mkInjections_1_injinc _ _ _ _ _ _ _ _ _ _ HeqMKI VBj12_1).
+  assert (inc12:= inc_RU _ _ preinc12 j').
+  assert (presep12:= mkInjections_1_injsep _ _ _ _ _ _ _ _ _ _ HeqMKI).
+  assert (sep12: inject_separated j12 (removeUndefs j12 j' prej12') m1 m2).
+       intros b; intros. eapply presep12. apply H. 
+       eapply RU_D. apply preinc12. apply H0.
+  assert (inc23:= mkInjections_2_injinc _ _ _ _ _ _ _ _ _ _ HeqMKI VBj23_1).
+  assert (sep23:= mkInjections_2_injsep _ _ _ _ _ _ _ _ _ _ HeqMKI 
+                  VBj12_1 _ InjSep).
+  assert (NB1: Mem.nextblock m1' - Mem.nextblock m1 >= 0).
+       assert (B: forall b, b <= Mem.nextblock m1 -> b <= Mem.nextblock m1'). 
+           intros. destruct (Fwd1 (b -1)).  unfold Mem.valid_block. omega. 
+                 unfold Mem.valid_block in H0. omega. 
+       clear -B. specialize (B (Mem.nextblock m1)). omega. 
+  destruct (mkInjectionsN_0  _ _ _ _ _ _ _ _ _ _ HeqMKI) as [N1 N2].
+       rewrite (nat_of_Z_eq _ NB1) in N1. 
+       rewrite (nat_of_Z_eq _ NB1) in N2. 
+       rewrite Zplus_minus in N1. subst.
+  assert (VBj': forall b1 b3 ofs3, j' b1 = Some (b3, ofs3) -> 
+                b1 < Mem.nextblock m1').
+      intros. apply (Mem.valid_block_inject_1 _ _ _ _ _ _ H MInj13').
+  assert (ID:= RU_composememinj _ _ _ _ _ _ _ _ _ _ HeqMKI 
+               InjIncr _ InjSep VBj12_1 VBj12_2 VBj23_1 VBj').
+  assert (preAL12' := mkInjections_aligned_1 _ _ _ _ _ _ _ _ _ _ HeqMKI AL12).
+  assert (AL12' : inject_aligned  (removeUndefs j12 j' prej12')).
+          intros b; intros. apply RU_D in H.  
+          eapply preAL12'. apply H. assumption.
+  assert (AL23' := mkInjections_aligned_2 _ _ _ _ _ _ _ _ _ _ 
+                   HeqMKI AL23 AL13').
+split. assumption.
+split. assumption.
+split. assumption.
+split. assumption.
+split. assumption.
+assert (IDextensional: forall b,  
+            j' b = compose_meminj (removeUndefs j12 j' prej12') j23' b).
+   intros. rewrite <- ID. trivial.
+clear ID.
+assert (Fwd2: mem_forward m2 m2').
+  split; intros; rename b into b2.
+  (*valid_block*)
+     clear - N2 H NB1. unfold Mem.valid_block in *. omega. 
+  (*max*)
+     destruct (ACCESS b2) as [Val2 _].
+     specialize (Val2 H Max ofs). 
+     remember (source j12 m1 b2 ofs) as src.
+     destruct src.
+       apply source_SomeE in Heqsrc.
+       destruct Heqsrc as [b1 [delta [ofs1 [PBO [Bounds [J1 [P1 Off2]]]]]]].
+       subst.
+       rewrite (perm_subst _ _ _ _ _ _ _ Val2) in H0; clear Val2.
+       rewrite (IP12 _ _ _ P1 _ _ J1).
+             eapply Fwd1.
+                apply (Mem.perm_valid_block _ _  _ _ _ P1).
+                apply H0.
+    rewrite (perm_subst _ _ _ _ _ _ _ Val2) in H0; clear Val2. apply H0.
+assert (Unch2: my_mem_unchanged_on (loc_out_of_reach j12 m1) m2 m2').
+  split; intros.
+     apply (valid_split _ _ _ _ (ACCESS b)); intros; clear ACCESS.
+     (* case Mem.valid_block m2 b*)
+        specialize (H1 k ofs).
+        remember (source j12 m1 b ofs) as d.
+        destruct d.
+           destruct p. 
+           rewrite (perm_subst _ _ _ _ _ _ _ H1). clear H1.
+           destruct (source_SomeE _ _ _ _ _ Heqd)
+              as [bb1 [dd1 [ofs11 [PP [VB [ JJ [PERM Off2]]]]]]]. clear Heqd.
+           subst. apply eq_sym in PP. inv PP.
+           specialize (HP _ _ JJ). assert (z + dd1 - dd1 = z). omega. 
+           rewrite H1 in HP.
+           exfalso. apply (HP PERM).
+         rewrite (perm_subst _ _ _ _ _ _ _ H1). trivial.
+      (*invalid*)
+           exfalso. apply (H0 H).
+  apply (valid_split _ _ _ _ (CONT b)); intros; clear CONT.
+      (* case Mem.valid_block m2 b*)
+          specialize (H1 ofs).
+          remember (source j12 m1 b ofs) as d.
+          destruct d.
+            destruct p.
+            destruct (source_SomeE _ _ _ _ _ Heqd)
+               as [bb1 [dd1 [ofs11 [PP [VB [ JJ [PERM Off2]]]]]]]. clear Heqd.
+            subst. apply eq_sym in PP. inv PP.
+            specialize (HP _ _ JJ).
+            assert (z + dd1 - dd1 = z). omega. 
+            rewrite H in HP.
+            exfalso. apply (HP  PERM).
+          rewrite  H1. trivial.
+       (*invalid*)
+          exfalso. apply Mem.perm_valid_block in HMeperm. apply (H0 HMeperm).
+assert (UnchLOM2: my_mem_unchanged_on (loc_unmapped j23) m2 m2').
+  unfold loc_unmapped.
+  split; intros.
+      apply (valid_split _ _ _ _ (ACCESS b)); intros; clear ACCESS.
+      (*case Mem.valid_block m2 b*)
+          specialize (H1 k ofs).
+          remember (source j12 m1 b ofs) as d.
+          destruct d.
+            destruct p. 
+            rewrite (perm_subst _ _ _ _ _ _ _ H1). clear H1.
+            destruct (source_SomeE _ _ _ _ _ Heqd)
+              as [bb1 [dd1 [ofs11 [PP [VB [ JJ [PERM Off2]]]]]]]. clear Heqd.
+            subst. apply eq_sym in PP. inv PP.
+            destruct Unch11'.
+            rewrite <- H1.
+               apply IP12. apply PERM. apply JJ.
+               unfold loc_unmapped, compose_meminj. rewrite JJ. 
+                  rewrite HP. trivial.
+               apply (Mem.perm_valid_block _ _ _ _ _ PERM).
+          rewrite (perm_subst _ _ _ _ _ _ _ H1). trivial.
+      (* case invalid*)
+          exfalso. apply (H0 H).
+  apply (valid_split _ _ _ _ (CONT b)); intros; clear CONT.
+      (*case Mem.valid_block m2 b*)
+          specialize (H1 ofs).
+          assert (j23' b = None).
+               remember (j23' b) as d.
+               destruct d; trivial. apply eq_sym in Heqd. destruct p.
+               destruct (sep23 _ _ _ HP Heqd). exfalso. apply (H2 H0).
+          remember (source j12 m1 b ofs) as d.
+          destruct d.
+             destruct p. subst. rewrite H2 in H1. apply H1. 
+          (* destruct (source_SomeE _ _ _ _ _ Heqd) 
+                   as [bb1 [dd1 [ofs11 [PP [VB [ JJ [PERM Off2]]]]]]]. 
+                 clear Heqd.
+                 subst. apply eq_sym in PP. inv PP. 
+                 unfold compose_meminj in H1. rewrite (inc12 _ _ _ JJ) in H1.
+                 rewrite H2 in H1. apply H1.*)
+          rewrite H1. apply H.
+      (*case invalid*)
+          exfalso. apply Mem.perm_valid_block in HMeperm. apply (H0 HMeperm).
+assert (UnchLOOR3: my_mem_unchanged_on (loc_out_of_reach j23 m2) m3 m3').
+   unfold loc_out_of_reach.
+   split; intros.
+      eapply Unch33'. 
+        unfold loc_out_of_reach, compose_meminj. intros.
+           remember ( j12 b0) as d.
+           destruct d. 
+              apply eq_sym in Heqd. destruct p.
+              remember (j23 b1) as dd.
+              destruct dd; inv H0. apply eq_sym in Heqdd. destruct p. inv H2.
+              specialize (HP _ _ Heqdd). 
+              intros N. apply HP.
+              rewrite <- (IP12 b0 _ Max N _ _ Heqd) in N.
+              assert (ofs - (z + z0) + z = ofs - z0). omega.
+              rewrite H0 in N. apply N.
+           inv H0.
+        apply H. 
+   eapply Unch33'. 
+        unfold loc_out_of_reach, compose_meminj. intros.
+           remember ( j12 b0) as d.
+           destruct d.
+              apply eq_sym in Heqd. destruct p.
+              remember (j23 b1) as dd.
+              destruct dd; inv H0. apply eq_sym in Heqdd. destruct p. inv H2.
+              specialize (HP _ _ Heqdd).
+              intros N. apply HP.
+              rewrite <- (IP12 b0 _ Max N _ _ Heqd) in N.
+              assert (ofs - (z + z0) + z = ofs - z0). omega.
+              rewrite H in N. apply N.
+           inv H0.
+        apply HMeperm.
+        apply H.
+assert (NOVj12':= RU_no_overlap _ _ _ MInj12 _ Fwd1 _ _ 
+                  MInj23 _ _ _ _ _ HeqMKI).
+assert (IP12': inject_perm_nonempty (removeUndefs j12 j' prej12') m1' m2').
+   intros b; intros.
+   apply (valid_split _ _ _ _ (ACCESS b2)); intros; clear ACCESS.
+   (*Mem.valid_block m2 b2*)
+       specialize (H0 k (ofs+delta)).
+       assert (FF: j12 b = Some (b2, delta)).
+             remember (j12 b) as dd.
+             destruct dd; apply eq_sym in Heqdd.
+                destruct p. apply inc12 in Heqdd. rewrite Heqdd in F. apply F.
+              destruct (sep12 _ _ _ Heqdd F).
+                 exfalso. apply (H2 H).
+       assert (ValB1:= VBj12_1 _ _ _ FF).
+          remember (source j12 m1 b2 (ofs+delta)) as d.
+          destruct d. destruct p. 
+             rewrite (perm_subst _ _ _ _ _ _ _ H0).
+             destruct (source_SomeE _ _ _ _ _ Heqd)
+                as [bb1 [dd1 [ofs11 [PP [VB [ JJ [PERM Off2]]]]]]]. clear Heqd.
+             subst. apply eq_sym in PP. inv PP.
+             assert (JJ' := preinc12 _ _ _ JJ).
+             destruct (eq_block b0 b); subst.
+                rewrite FF in JJ. inv JJ. 
+                assert (ofs = z). omega. subst. trivial.
+             specialize (Mem.mi_no_overlap _ _ _ MInj12). intros NOV.
+                 apply (Fwd1 _ ValB1) in NP.
+                 destruct (NOV b0 b2 dd1 b b2 delta z ofs n JJ FF PERM NP).
+                    exfalso. apply H1. trivial.
+                    exfalso. rewrite Off2 in H1. apply H1. trivial.
+       rewrite (perm_subst _ _ _ _ _ _ _ H0). clear H0.
+          assert (SRC:=  sourceNone_LOOR _ _ _ _ Heqd _ MInj12 _ _ FF). 
+          clear Heqd.
+          assert (ofs + delta - delta = ofs). omega. 
+          rewrite H0 in SRC.
+          exfalso. apply (Fwd1 _ ValB1) in NP. apply (SRC NP).
+   (*case invalid*)
+       specialize (H0 k (ofs+delta)).
+       assert (J12: j12 b = None).
+           remember (j12 b) as d.
+           destruct d; trivial. apply eq_sym in Heqd. destruct p.
+              assert (X:= VBj12_2 _ _ _ Heqd).
+              apply inc12 in Heqd. rewrite Heqd in F.  inv F. 
+              exfalso.  apply (H X).
+       remember (source (removeUndefs j12 j' prej12') m1' b2 (ofs+delta)) as d.
+       destruct d.
+          destruct p.
+          rewrite (perm_subst _ _ _ _ _ _ _ H0).
+          destruct (source_SomeE _ _ _ _ _ Heqd)
+            as [bb1 [dd1 [ofs11 [PP [VB [ JJ' [PERM Off2]]]]]]]. clear Heqd.
+          subst. apply eq_sym in PP. inv PP.
+          destruct (eq_block b0 b); subst.
+             rewrite F in JJ'. inv JJ'.
+             assert (ofs = z). omega. 
+             subst. trivial. 
+          destruct (NOVj12' b0 b2 dd1 b b2 delta z ofs n JJ' F PERM NP). 
+                     exfalso. apply H1. trivial.
+                     exfalso. rewrite Off2 in H1. apply H1. trivial.
+       specialize (source_NoneE _ _ _ _ Heqd). intros SRC. clear Heqd.
+          assert (Val1' := Mem.perm_valid_block _ _ _ _ _ NP).
+          specialize (SRC _ _  (VALIDBLOCK _ _ Val1') F). 
+          assert (ofs + delta - delta = ofs). omega. 
+          rewrite H1 in SRC. exfalso. apply (SRC NP).
+assert (IP23': inject_perm_nonempty j23' m2' m3'). clear CONT.
+   intros b; intros.
+   apply (valid_split _ _ _ _ (ACCESS b)); intros; clear ACCESS.
+   (*case Mem.valid_block m2 b*)
+       assert (P2':= H0 Max ofs).
+       specialize (H0 k ofs).
+       assert (FF: j23 b = Some (b2, delta)).
+            remember (j23 b) as dd.
+            destruct dd; apply eq_sym in Heqdd.
+               destruct p. apply inc23 in Heqdd. rewrite Heqdd in F. apply F.
+            destruct (sep23 _ _ _ Heqdd F). exfalso. apply (H1 H).
+       remember (source j12 m1 b ofs) as d.
+       destruct d. 
+       (*source  j12 m1 b ofs = Some*)
+           destruct p. 
+           rewrite (perm_subst _ _ _ _ _ _ _ H0). clear H0.
+           rewrite (perm_subst _ _ _ _ _ _ _ P2') in NP. clear P2'.
+           destruct (source_SomeE _ _ _ _ _ Heqd)
+              as [bb1 [dd1 [ofs11 [PP [VB [ JJ [PERM Off2]]]]]]]. clear Heqd.
+           subst. apply eq_sym in PP. inv PP.
+           assert (JJ': j' b0 = Some (b2, dd1 + delta)). 
+                 rewrite IDextensional. 
+                 unfold compose_meminj. rewrite (inc12 _ _ _ JJ). 
+                 rewrite F. trivial.
+           rewrite <- Zplus_assoc.
+           eapply (IPj' b0 _ k NP). apply JJ'.
+       (*source  j12 m1 b ofs = None*)
+           rewrite (perm_subst _ _ _ _ _ _ _ H0). clear H0.
+           rewrite (perm_subst _ _ _ _ _ _ _ P2') in NP. clear P2'.
+           assert (SRC:= source_NoneE _ _ _ _ Heqd). clear Heqd.
+           assert (UNCH: loc_out_of_reach (compose_meminj j12 j23) 
+                         m1 b2 (ofs + delta)).
+                 unfold loc_out_of_reach, compose_meminj. intros.
+                 remember (j12 b0) as dd.
+                 destruct dd; inv H0. 
+                 destruct p. apply eq_sym in Heqdd.   
+                 remember (j23 b1) as ddd.
+                 destruct ddd; inv H2.
+                 destruct p. apply eq_sym in Heqddd. inv H1.
+                 destruct (eq_block b1 b); subst.
+                      rewrite Heqddd in FF. inv FF. 
+                      assert (ofs + delta - (z + delta) = ofs - z). omega. 
+                      rewrite H0.
+                      apply (SRC _ _ (VALIDBLOCK _ _ 
+                                    (VBj12_1 _ _ _ Heqdd)) Heqdd).
+                 intros N. 
+                 assert (PX:Mem.perm m2 b1 (ofs+delta-z0) Max Nonempty).
+                       rewrite <- (IP12 b0 _ Max N _ _ Heqdd) in N.
+                       assert (ofs + delta - (z + z0) + z = 
+                                    ofs + delta - z0). omega. 
+                       rewrite H0 in N. apply N.
+                 assert (NOV := Mem.mi_no_overlap _ _ _ 
+                              MInj23 b1 _ _ b _ _ _ _ n Heqddd FF PX NP).
+                 destruct NOV. 
+                    apply H0. trivial.
+                    apply H0. omega.
+           destruct Unch33' as [U33P _]. 
+             rewrite <- U33P. 
+                eapply IP23. apply NP.  apply FF. 
+                apply UNCH.
+                apply (VBj23_2 _ _ _ FF).
+   (*case invalid*)
+        assert (Max2':= H0 Max ofs).
+        specialize (H0 k ofs).
+        assert (J12: j23 b = None).
+                remember (j23 b) as d.
+                destruct d; trivial. apply eq_sym in Heqd. destruct p.
+                assert (X:= VBj23_1 _ _ _ Heqd).
+                exfalso.  apply (H X).
+        remember ( source (removeUndefs j12 j' prej12') m1' b ofs) as d.
+        destruct d. 
+          destruct p.
+          rewrite (perm_subst _ _ _ _ _ _ _ H0) in*. clear H0.
+          rewrite (perm_subst _ _ _ _ _ _ _ Max2') in*. clear Max2'.
+          destruct (source_SomeE _ _ _ _ _ Heqd)
+             as [bb1 [dd1 [ofs11 [PP [VB [ JJ' [PERM Off2]]]]]]]. clear Heqd.
+          subst. apply eq_sym in PP. inv PP.
+          rewrite <- Zplus_assoc.
+          eapply IPj'. apply PERM.
+          rewrite IDextensional.
+          unfold compose_meminj. rewrite JJ'. rewrite F. trivial.
+        unfold Mem.perm in NP. rewrite Max2' in NP. inv NP.
+assert (Inj12': Mem.inject (removeUndefs j12 j' prej12')  m1' m2').
+    assert (Perm12': forall b1 b2 delta ofs k p,
+             (removeUndefs j12 j' prej12') b1 = Some (b2, delta) ->
+             Mem.perm m1' b1 ofs k p -> Mem.perm m2' b2 (ofs + delta) k p).
+        intros.
+        apply (valid_split _ _ _ _ (ACCESS b2)); intros; clear ACCESS.
+        (*case valid_block m2 b2*)
+            specialize (H2 k (ofs+delta)).
+            remember (j12 b1) as d.
+            destruct d; apply eq_sym in Heqd.
+               destruct p0 as [bb dd]. rewrite (inc12 _ _ _ Heqd) in H. inv H.
+               rewrite (source_SomeI j12 _  _ b1) in H2.
+               rewrite (perm_subst _ _ _ _ _ _ _ H2). apply H0.
+               apply MInj12.
+               assumption.
+               apply Fwd1. apply (VBj12_1 _ _ _ Heqd). 
+                           eapply Mem.perm_implies. eapply Mem.perm_max. 
+                               apply H0. apply perm_any_N.
+            destruct (sep12 _ _ _ Heqd H) as [_ NV2]. exfalso. apply (NV2 H1).
+        (*case ~ valid_block m2 b2*)
+            specialize (H2 k (ofs+delta)).
+            rewrite (source_SomeI (removeUndefs j12 j' prej12') _  _ b1) in H2.
+            rewrite (perm_subst _ _ _ _ _ _ _ H2). apply H0.
+            apply (RU_no_overlap _ _ _ MInj12 _ Fwd1 _ _ 
+                    MInj23 _ _ _ _ _ HeqMKI).
+               assumption.
+               eapply Mem.perm_implies. eapply Mem.perm_max. 
+                    apply H0. apply perm_any_N.
+    assert (INJ:Mem.mem_inj  (removeUndefs j12 j' prej12') m1' m2'). 
+      split. apply Perm12'.
+      (*valid_access*) 
+          intros. destruct H0.
+          split.
+              intros off; intros.
+              assert (Hoff: ofs <= off-delta < ofs + size_chunk chunk). omega. 
+              specialize (Perm12' _ _ _ _ _ _ H  (H0 _ Hoff)).
+              assert (off - delta + delta = off). omega. 
+              rewrite H3 in Perm12'. apply Perm12'.
+              (*we can't use Mem.aligned_area_inject because we want to 
+                PROVE Mem.inject (removeUndefs j12 j' prej12')  m1' m2').*)
+                (*assert (RP : Mem.range_perm m1' b1 ofs 
+                              (ofs + size_chunk chunk) Cur Nonempty).
+                  intros off Hoff. eapply Mem.perm_implies.
+                    apply (H0 _ Hoff). apply perm_any_N. 
+                   eapply Mem.aligned_area_inject with
+                    (sz:=size_chunk chunk). Focus 5. apply RP. 
+                        Focus 6. apply H. 
+                            apply H1. Focus 4. apply H1.
+                  THIS IS ONE OF THE PLACES WHERE 
+                       inject_aligned_of IS REQUIRED*)
+                   eapply (inject_aligned_ofs _ AL12' _ _ _ _ H _ H1). 
+      (*memval  j12' m1' m2'.*)
+          intros. 
+          apply (valid_split _ _ _ _ (CONT b2)); intros; clear CONT.
+         (*case Mem.valid_block m2 b2*)
+             specialize (H2 (ofs + delta)).
+             assert (J12:  j12 b1 = Some (b2, delta)).
+                 remember (j12 b1) as d. 
+                 destruct d; apply eq_sym in Heqd.
+                      destruct p. rewrite (inc12 _ _ _ Heqd) in H. apply H.
+                      destruct (sep12 _ _ _ Heqd H). exfalso. apply (H4 H1).
+             assert (Val1:= VBj12_1 _ _ _ J12).
+             assert (Perm1: Mem.perm m1 b1 ofs Max Nonempty).
+                   apply (Fwd1 _ Val1). 
+                      eapply Mem.perm_max. eapply Mem.perm_implies.
+                        apply H0. apply perm_any_N.
+             remember (source j12 m1 b2 (ofs + delta)) as ss.
+             destruct ss.
+             (*source  j12 m1 b2 (ofs + delta)  = Some p *)
+                 destruct (source_SomeE _ _ _ _ _ Heqss)
+                    as [bb1 [dd1 [ofs11 [PP [VB [ JJ [PERM Off2]]]]]]].
+                 clear Heqss. subst.     
+                 destruct (eq_block bb1 b1); subst.
+                 (*case bb1 = b1*)
+                     rewrite J12 in JJ. apply eq_sym in JJ. inv JJ. 
+                     assert (ofs11 = ofs). omega. 
+                     subst. clear Off2. 
+                     remember (j23' b2) as j23'b2.
+                     destruct j23'b2; apply eq_sym in Heqj23'b2.
+                     (*j23' b2 = Some p*)
+                         destruct p. rewrite H2. clear H2.
+                         assert (COMP: compose_meminj 
+                                   (removeUndefs j12 j' prej12') j23' b1 = 
+                                 Some(b, delta+z)).
+                            unfold compose_meminj. rewrite H. 
+                            rewrite Heqj23'b2. trivial.
+                         assert (COMP': j' b1 = Some(b, delta+z)). 
+                            rewrite IDextensional. apply COMP.
+                         assert (MV:= Mem.mi_memval _ _ _
+                            (Mem.mi_inj _ _ _ MInj13') _ _  _ _ COMP' H0).
+                         inv MV; try constructor. 
+                           simpl. 
+                           rewrite IDextensional in H4.
+                           apply compose_meminjD_Some in H4.
+                           destruct H4 as [bb1 [off1 [off [JJ1 [JJ2 Delta]]]]].
+                           subst. 
+                           rewrite JJ1. econstructor. apply JJ1. trivial.
+                     (*j23' b2 = None*)
+                         rewrite H2. clear H2.
+                         assert (J23: j23 b2 = None).
+                            remember (j23 b2) as d; 
+                            destruct d; trivial; apply eq_sym in Heqd.
+                            destruct p. 
+                            rewrite (inc23 _ _ _ Heqd) in Heqj23'b2. 
+                            discriminate.
+                         destruct Unch11' as [Uperm Uval]. 
+                         assert (UNMAPPED: loc_unmapped 
+                                       (compose_meminj j12 j23) b1 ofs).
+                            unfold compose_meminj, loc_unmapped. 
+                            rewrite J12. rewrite J23. trivial.
+                         assert (RD: Mem.perm m1 b1 ofs Cur Readable). 
+                            rewrite Uperm. assumption. assumption. assumption.
+                         rewrite (Uval b1 ofs UNMAPPED RD _ (eq_refl _)).
+                         apply (memval_inject_incr j12).
+                            apply (Mem.mi_memval _ _ _ 
+                               (Mem.mi_inj _ _ _ MInj12) _ _  _ _ J12 RD).
+                            assumption.
+                 (* case bb1 <> b1*)   
+                      exfalso. 
+                      destruct (Mem.mi_no_overlap _ _ _ MInj12
+                             bb1 _ _ _ _ _ _ _ n JJ J12 PERM  Perm1).
+                        apply H3; trivial.
+                        apply H3. rewrite Off2. trivial.
+             (*source  j12 m1 b2 (ofs + delta)  = None *)
+                 exfalso.
+                 apply (source_NoneE _ _ _ _ Heqss _ _  
+                        (VALIDBLOCK _ _ Val1) J12). 
+                 assert (ofs + delta - delta = ofs). omega.
+                 rewrite H3. apply Perm1.  
+         (*case ~ Mem.valid_block m2 b2*)
+            specialize (H2 (ofs + delta)).
+            assert (J12:  j12 b1 = None).
+               remember (j12 b1) as d. 
+               destruct d; apply eq_sym in Heqd; trivial.
+                     destruct p. rewrite (inc12 _ _ _ Heqd) in H. inv H.
+                     exfalso. apply H1. apply (VBj12_2 _ _ _ Heqd).
+            remember (source  (removeUndefs j12 j' prej12')
+                   m1' b2 (ofs + delta)) as ss.
+            destruct ss.
+            (*source  j12' m1' b2 (ofs + delta)  = Some p *)
+                destruct p. rewrite H2. clear H2.
+                remember (ZMap.get ofs (ZMap.get b1 (Mem.mem_contents m1'))) 
+                          as v.
+                destruct (source_SomeE _ _ _ _ _ Heqss)
+                      as [bb1 [dd1 [ofs11 [PP [VB [ JJ [PERM Off2]]]]]]].
+                clear Heqss.
+                apply eq_sym in PP. inv PP.
+                assert (MX: Mem.perm m1' b1 ofs Max Nonempty).
+                    eapply Mem.perm_max. eapply Mem.perm_implies.
+                    apply H0. apply perm_any_N.
+                destruct (eq_block b b1); subst.
+                (*case b = b1*)
+                   rewrite H in JJ. apply eq_sym in JJ. inv JJ. 
+                   assert (z = ofs). omega. 
+                   subst.  clear Off2. 
+                   remember (ZMap.get ofs (ZMap.get b1 (Mem.mem_contents m1')))
+                              as v.
+                   remember (j23' b2) as j23'b2.
+                   destruct j23'b2; apply eq_sym in Heqj23'b2.
+                   (*j23' b2 = Some p*)
+                       destruct p as [b3 delta3].
+                       assert (COMP: compose_meminj 
+                                  (removeUndefs j12 j' prej12') j23' b1
+                                  = Some(b3, delta+delta3)).
+                           unfold compose_meminj. 
+                           rewrite H. rewrite Heqj23'b2. trivial.
+                       assert (COMP': j' b1 = Some(b3, delta+delta3)).
+                            rewrite IDextensional. apply COMP.
+                       assert (MV:= Mem.mi_memval _ _ _ 
+                           (Mem.mi_inj _ _ _ MInj13') _ _  _ _ COMP' H0).
+                       subst. (*revert the abbreviation v that was
+                            introduced for "self-didactic" purpose*)
+                       inv MV; try constructor. 
+                       simpl. rewrite IDextensional in H4. 
+                       apply compose_meminjD_Some in H4.
+                       destruct H4 as [bb1 [off1 [off [JJ1 [JJ2 Delta]]]]].
+                       subst. 
+                       rewrite JJ1. econstructor. apply JJ1. trivial.
+                   (*j23' b2 = None -- the following 5 lines are where the
+                         removeUndefs definition comes into play
+                         (compare to MemoryPsuhout_II_Wrong!)
+                         probably the is can be cleaned up a bit...!*)
+                       clear - IDextensional H J12 Heqj23'b2.
+                       unfold removeUndefs in H. rewrite J12 in H.
+                       remember (j' b1) as d.
+                       destruct d; try inv H. 
+                       destruct p. rewrite IDextensional in Heqd.
+                       unfold compose_meminj, removeUndefs in Heqd. 
+                       rewrite J12 in Heqd. 
+                       remember ( j' b1) as d.
+                       destruct d. 
+                         destruct p. rewrite H1 in Heqd. 
+                         rewrite Heqj23'b2 in Heqd.  inv Heqd.
+                       inv Heqd.
+                (* case b <> b1*)  exfalso. 
+                    destruct (NOVj12' b  _ _ _ _ _ _ _ n JJ H PERM MX).
+                         apply H2; trivial.
+                         apply H2. rewrite Off2. trivial.
+            (*source  j12' m1' b2 (ofs + delta)  = None *) exfalso.
+               apply (source_NoneE _ _ _ _ Heqss _ _ 
+                    (VALIDBLOCK _ _  (Mem.perm_valid_block _ _ _ _ _ H0)) H). 
+               assert (ofs + delta - delta = ofs). omega.
+               rewrite H3.
+               eapply Mem.perm_max. eapply Mem.perm_implies.
+                    apply H0. apply perm_any_N.
+   split. apply INJ.
+   (* mi_freeblocks*)  intros. 
+        remember (removeUndefs j12 j' prej12'  b) as d.
+        destruct d; apply eq_sym in Heqd; trivial. destruct p.
+        unfold removeUndefs in Heqd.
+        remember (j12 b) as dd.
+        destruct dd; apply eq_sym in Heqdd.
+            destruct p.
+            exfalso. apply H. apply Fwd1. apply (VBj12_1 _ _ _ Heqdd).
+        remember (j' b) as ddd.
+        destruct ddd; apply eq_sym in Heqddd.
+            destruct p. exfalso. apply H. apply (VBj' _ _ _ Heqddd).
+        inv Heqd.
+  (*mi_mappedblock*) intros.
+     assert (ValJ12: forall b1 b2 ofs2,  j12 b1 = Some (b2, ofs2) ->
+                     b1 < Mem.nextblock m1 /\ b2 < Mem.nextblock m2).
+         intros. split. apply (VBj12_1 _ _ _ H0). apply (VBj12_2 _ _ _ H0).
+     remember (removeUndefs j12 j' prej12'  b) as d.
+     destruct d; apply eq_sym in Heqd.
+        inv H.
+        unfold removeUndefs in Heqd.
+        remember (j12 b) as dd.
+        destruct dd; apply eq_sym in Heqdd.
+            destruct p. inv Heqd. apply Fwd2. apply (VBj12_2 _ _ _ Heqdd).
+        remember (j' b) as ddd.
+        destruct ddd; apply eq_sym in Heqddd.
+          destruct p. 
+          destruct (mkInjectionsN_3V _ _ _ _ _ _ _ _ _ _ 
+                      HeqMKI ValJ12  VBj23_1 _ _ _ Heqd).
+            destruct H as [J12 [Val1 Val2]]. apply Fwd2. apply Val2.
+            destruct H as [? [_ [_ [_ [_ [_ D]]]]]]. apply D.
+        inv Heqd.
+     inv H.
+  (*no_overlap*)
+       apply (RU_no_overlap _ _ _ MInj12 _ Fwd1 _ _ MInj23 _ _ _ _ _ HeqMKI).
+  (*representable*)
+       intros. 
+       unfold removeUndefs in H.
+       remember (j12 b) as d.
+       destruct d; apply eq_sym in Heqd.
+          destruct p0. inv H.
+          eapply MInj12. apply Heqd. 
+          apply Fwd1. apply (VBj12_1 _ _ _ Heqd). eapply Mem.perm_max. apply H0.
+       remember (j' b) as dd.
+       destruct dd; apply eq_sym in Heqdd.
+          destruct p0.
+          destruct (mkInjectionsN_3V _ _ _ _ _ _ _ _ _ _ 
+                     HeqMKI VB12  VBj23_1 _ _ _ H).
+              destruct H1. rewrite H1 in Heqd. discriminate.
+              destruct H1 as [M [ZM [A [B [C [D E]]]]]]. 
+                 rewrite C in *.
+                 split. omega. 
+                        rewrite Zplus_0_r. apply Int.unsigned_range_2.
+       inv H.  
+split; trivial.
+split; trivial.
+assert (Inj23': Mem.inject j23' m2' m3').
+   assert (Perm23': forall b1 b2 delta ofs k p,
+                j23' b1 = Some (b2, delta) -> 
+                Mem.perm m2' b1 ofs k p -> Mem.perm m3' b2 (ofs + delta) k p).
+      intros b2 b3; intros. 
+      apply (valid_split _ _ _ _ (ACCESS b2)); intros; clear ACCESS.
+      (*valid*)
+          specialize (H2 k ofs).
+          assert (FF: j23 b2 = Some (b3, delta)).
+             remember (j23 b2) as dd.
+             destruct dd; apply eq_sym in Heqdd.
+               destruct p0. apply inc23 in Heqdd. rewrite Heqdd in H. apply H.
+             destruct (sep23 _ _ _ Heqdd H). exfalso. apply (H3 H1).
+          remember (source j12 m1 b2 ofs) as d.
+          destruct d. 
+          (*source  j12 m1 b2 ofs = Some p0*)
+              destruct p0. 
+              destruct (source_SomeE _ _ _ _ _ Heqd)
+                 as [bb1 [dd1 [ofs11 [PP [VB [ JJ [PERM Off2]]]]]]]. clear Heqd.
+              subst. apply eq_sym in PP. inv PP.
+              rewrite (perm_subst _ _ _ _ _ _ _ H2) in H0. clear H2.
+              rewrite <- Zplus_assoc.
+              rewrite (IPj' b). 
+                 apply H0.
+                 eapply Mem.perm_max. eapply Mem.perm_implies. 
+                       apply H0. apply perm_any_N.
+                eapply InjIncr. unfold compose_meminj. 
+                                rewrite JJ. rewrite FF. trivial.
+          (*source  j12 m1 b2 ofs = None*)
+              rewrite (perm_subst _ _ _ _ _ _ _ H2) in H0. clear H2.
+              assert (MX: Mem.perm m2 b2 ofs Max Nonempty).
+                  eapply Mem.perm_max. eapply Mem.perm_implies.
+                     apply H0. apply perm_any_N.
+              assert (SRC:= source_NoneE _ _ _ _ Heqd). clear Heqd.
+              assert (UNCH: loc_out_of_reach 
+                          (compose_meminj j12 j23) m1 b3 (ofs + delta)).
+                  unfold loc_out_of_reach, compose_meminj. intros.
+                  remember (j12 b0) as dd.
+                  destruct dd; inv H2. 
+                  destruct p0. apply eq_sym in Heqdd.   
+                  remember (j23 b) as ddd.
+                  destruct ddd; inv H4. 
+                  destruct p0. apply eq_sym in Heqddd. inv H3.
+                  destruct (eq_block b2 b); subst.
+                  (*case b2=b*)
+                     rewrite (inc23 _ _ _ Heqddd) in H. inv H. 
+                     assert (ofs + delta - (z + delta) = ofs - z). omega. 
+                     rewrite H.
+                     apply (SRC _ _ (VALIDBLOCK _ _  
+                                          (VBj12_1 _ _ _ Heqdd)) Heqdd).
+                  (*case b2 <> b*)
+                     intros N. 
+                     assert (PX: Mem.perm m2 b (ofs + delta - z0) Max Nonempty).
+                        rewrite <- (IP12 b0 _ Max N _ _ Heqdd) in N.
+                        assert (ofs+delta-(z+z0)+z = ofs+delta-z0). omega. 
+                        rewrite H2 in N. apply N.
+                     assert (NOV := Mem.mi_no_overlap _ _ _ 
+                            MInj23 b2 _ _ b _ _ _ _ n FF Heqddd MX PX).
+                     destruct NOV.
+                           apply H2. trivial.
+                           apply H2. omega.
+              destruct Unch33' as [U33P _]. 
+              rewrite <- U33P. 
+                    rewrite (IP23 b2). apply H0.  apply MX. apply FF. 
+                    apply UNCH.
+                    apply (VBj23_2 _ _ _ FF).
+      (*invalid*)
+          assert (MX: Mem.perm m2' b2 ofs Max Nonempty).
+              eapply Mem.perm_max. eapply Mem.perm_implies. 
+                apply H0. apply perm_any_N.
+          assert (Max2':= H2 Max ofs).
+          specialize (H2 k ofs).
+          assert (J12: j23 b2 = None).
+              remember (j23 b2) as d.
+              destruct d; trivial. apply eq_sym in Heqd. destruct p0.
+              assert (X:= VBj23_1 _ _ _ Heqd).
+              exfalso.  apply (H1 X).
+          remember (source (removeUndefs j12 j' prej12') m1' b2 ofs) as d.
+          destruct d. destruct p0.
+              rewrite (perm_subst _ _ _ _ _ _ _ H2) in*. clear H2.
+              rewrite (perm_subst _ _ _ _ _ _ _ Max2') in*. clear Max2'.
+              destruct (source_SomeE _ _ _ _ _ Heqd)
+                as [bb1 [dd1 [ofs11 [PP [VB [ JJ' [PERM Off2]]]]]]]. clear Heqd.
+              subst. apply eq_sym in PP. inv PP.
+              rewrite <- Zplus_assoc.
+              rewrite (IPj' b).
+                  apply H0.
+                  apply PERM.
+                  rewrite IDextensional. unfold compose_meminj.
+                           rewrite JJ'. rewrite H. trivial.
+          unfold Mem.perm in MX. rewrite Max2' in MX.  inv MX. 
+                      (*specialize (source_NoneE _ _ _ _ Heqd). intros SRC. clear Heqd.
+                        rewrite H in *.
+                        rewrite (perm_subst _ _ _ _ _ _ _ H2) in*. clear H2. trivial.*)
+   assert (MI: Mem.mem_inj j23' m2' m3').
+      split.
+      (*mi_perm *) apply Perm23'.
+      (*valid_access*)
+          intros. destruct H0.
+          split. intros off; intros. 
+                 assert (ofs <= off - delta < ofs + size_chunk chunk). omega.
+                 specialize (H0 _ H3).
+                 specialize (Perm23' _ _ _ _ _ _ H H0).
+                 assert (off - delta + delta = off). omega. 
+               rewrite H4 in Perm23'. apply Perm23'.
+          eapply (inject_aligned_ofs _ AL23' _ _ _ _ H _ H1). 
+      (*memval j23' m2' m3'*) intros b2 ofs2 b3 delta3 Jb2 Perm2.
+          assert (Perm2Max: Mem.perm m2' b2 ofs2  Max Nonempty).
+             eapply Mem.perm_max. eapply Mem.perm_implies.
+                        apply Perm2. constructor.
+          destruct (ACCESS b2) as [Valid Invalid].
+          apply (valid_split _ _ _ _ (CONT b2)); intros; clear CONT.
+          (*case Mem.valid_block m2 b2*)
+             specialize (Valid H Cur ofs2). clear Invalid.
+             specialize (H0 ofs2).
+             assert (J23:  j23 b2 = Some (b3, delta3)).
+                 remember (j23 b2) as d. destruct d; apply eq_sym in Heqd.
+                    destruct p. rewrite (inc23 _ _ _ Heqd) in Jb2. apply Jb2.
+                    destruct (sep23 _ _ _ Heqd Jb2). exfalso. apply (H1 H).
+             remember (source j12 m1 b2 ofs2) as ss.
+             destruct ss.
+             (*source  j12 m1 b2 ofs2  = Some p *)
+                destruct (source_SomeE _ _ _ _ _ Heqss)
+                    as [b1 [delta2 [ofs1 [PP [Valb1 [ Jb1 [Perm1 Off]]]]]]].
+                clear Heqss; subst.
+                rewrite (perm_subst _ _ _ _ _ _ _ Valid) in Perm2. clear Valid.
+                rewrite Jb2 in H0.
+                rewrite H0 in *. clear H0. simpl in *.
+                assert (Perm1'Max: Mem.perm m1' b1 ofs1 Max Nonempty).
+                   eapply Mem.perm_max. eapply Mem.perm_implies.
+                      apply Perm2. constructor.
+                assert (J': j' b1 = Some (b3, delta2 + delta3)).
+                    rewrite IDextensional. unfold compose_meminj. 
+                    rewrite (inc12 _ _ _ Jb1). rewrite Jb2. trivial.
+                specialize (Mem.mi_memval j' m1' m3'
+                    (Mem.mi_inj _ _ _ MInj13') _ _  _ _ J' Perm2). 
+                intros MemVal13'. 
+                rewrite IDextensional in J'.                   
+                destruct (compose_meminjD_Some _ _ _ _ _ J') 
+                    as [bb2 [dd2 [dd3 [RR [JJ23  DD]]]]]; subst.
+                assert (XX:= inc12 _ _ _ Jb1). rewrite RR in XX. inv XX. 
+                assert (dd3 = delta3). omega. 
+                rewrite H0 in *. clear H0 DD.
+                rewrite <- Zplus_assoc.
+                inv MemVal13'; simpl in *; try econstructor.
+                rewrite IDextensional in H2.                     
+                destruct (compose_meminjD_Some _ _ _ _ _ H2)
+                    as [bb2 [dd2 [ddd3 [RRR [JJJ23  DD]]]]]; subst.
+                rewrite RRR. econstructor. apply JJJ23.
+                rewrite Int.add_assoc. decEq. unfold Int.add. 
+                    apply Int.eqm_samerepr. auto with ints.
+             (*case source  j12 m1 b2 ofs2  = None *)
+                rewrite H0. clear H0.
+                rewrite (perm_subst _ _ _ _ _ _ _ Valid) in Perm2. clear Valid. 
+                assert (MX : Mem.perm m2 b2 ofs2 Max Nonempty).
+                     eapply Mem.perm_max. eapply Mem.perm_implies. 
+                     apply Perm2. constructor.
+                assert (LOOR: loc_out_of_reach 
+                             (compose_meminj j12 j23) m1 b3 (ofs2+delta3)).
+                     unfold loc_out_of_reach, compose_meminj. intros.
+                     remember (j12 b0) as q.
+                     destruct q; apply eq_sym in Heqq; inv H0.
+                     destruct p.
+                     remember (j23 b) as qq.
+                     destruct qq; apply eq_sym in Heqqq; inv H2. 
+                     destruct p. inv H1.
+                     destruct (eq_block b2 b); subst.
+                     (*case b2=b*)
+                         rewrite J23  in Heqqq. inv Heqqq. 
+                         assert (ofs2 + z0 - (z + z0) = ofs2 - z). omega. 
+                         rewrite H0.
+                         apply (source_NoneE _ _ _ _ Heqss). 
+                             apply (VALIDBLOCK _ _  (VBj12_1 _ _ _ Heqq)).
+                             apply Heqq.
+                     (*case b2<>b*)
+                         intros N.
+                         assert (NN2: Mem.perm m2 b
+                                     (ofs2 + (delta3 - z0)) Max Nonempty).
+                             rewrite <- (IP12 b0 _ Max N _ _ Heqq) in N.
+                             assert (ofs2 + delta3 - (z + z0) + z = 
+                                      ofs2 + (delta3 - z0)). omega. 
+                             rewrite H0 in N. apply N.
+                         destruct (Mem.mi_no_overlap _ _ _ 
+                                 MInj23 b2 _ _ b _ _ _ _ n J23 Heqqq MX NN2).
+                                     apply H0; trivial.
+                                     apply H0. omega.
+                assert (Perm3: Mem.perm m3 b3 (ofs2+delta3) Cur Readable).
+                   rewrite (IP23 b2). apply Perm2. apply MX. assumption.
+                destruct Unch33' as [Uperm UVal].
+                rewrite (UVal _ _ LOOR Perm3 _ (eq_refl _)).
+                eapply memval_inject_incr. 
+                  apply (Mem.mi_memval _ _ _ 
+                            (Mem.mi_inj _ _ _  MInj23) _ _ _ _ J23 Perm2). 
+                  apply inc23.
+          (*case ~ Mem.valid_block m2 b2*)
+             specialize (H0 ofs2). clear Valid.
+             assert (InvalidMax := Invalid H Max ofs2). 
+             specialize (Invalid H Cur ofs2).
+             assert (J23:  j23 b2 = None).
+                 remember (j23 b2) as d. 
+                 destruct d; apply eq_sym in Heqd; trivial.
+                    destruct p. rewrite (inc23 _ _ _ Heqd) in Jb2. inv Jb2.
+                          exfalso. apply H. apply (VBj23_1 _ _ _ Heqd).
+             remember (source (removeUndefs j12 j' prej12') m1' b2 ofs2) as ss.
+             destruct ss.
+             (*source  j12' m1' b2 ofs2  = Some p *)
+                 destruct p. rewrite H0 in *. clear H0.
+                 rewrite (perm_subst _ _ _ _ _ _ _ Invalid) in Perm2. 
+                 clear Invalid. 
+                 destruct (source_SomeE _ _ _ _ _ Heqss)
+                    as [b1 [delta2 [ofs1 [PP [VB [RR1 [Perm1' Off2]]]]]]].
+                 clear Heqss.
+                 inv PP.
+                 assert (Perm1'Max: Mem.perm m1' b1 ofs1 Max Nonempty).
+                   eapply Mem.perm_max. eapply Mem.perm_implies.
+                       apply Perm2. apply perm_any_N.
+                 assert (JB: j' b1 = Some (b3, delta2 + delta3)).
+                       rewrite IDextensional. unfold compose_meminj.
+                       rewrite RR1. rewrite Jb2. trivial.
+
+                 specialize (Mem.mi_memval _ _ _ 
+                       (Mem.mi_inj _ _ _  MInj13') _ _  _ _ JB Perm2). 
+                 intros MemVal13'.                    
+                 rewrite <- Zplus_assoc. 
+                 inv MemVal13'; simpl in *; try econstructor.
+                 rewrite IDextensional in H2.                     
+                 destruct (compose_meminjD_Some _ _ _ _ _ H2)
+                       as [bb2 [dd2 [ddd3 [RRR [JJJ23  DD]]]]]; subst.
+                    rewrite RRR. econstructor. apply JJJ23.
+                    rewrite Int.add_assoc. decEq. unfold Int.add. 
+                       apply Int.eqm_samerepr. auto with ints.  
+             (*source  j12' m1' b1 ofs  = None *) 
+                 unfold Mem.perm in Perm2. rewrite Invalid in Perm2. inv Perm2.
+   split; trivial.
+   (*mi_freeblocks*)
+       intros. remember (j23' b) as d.
+       destruct d; apply eq_sym in Heqd; trivial.
+       destruct p. exfalso.
+       specialize (mkInjectionsN_0 _ _ _ _ _ _ _ _ _ _ HeqMKI).
+       intros. destruct H0. clear H0.
+       rewrite nat_of_Z_eq in H1.
+         destruct (mkInjectionsN_4Val _ _ _ _ _ _ _ _ _ _ 
+             HeqMKI VBj23_1 _ _ _ Heqd).
+                      destruct H0. apply H. unfold Mem.valid_block. omega. 
+                      destruct H0 as [M [ZM [BM [J' B']]]].  apply (H B').
+         assumption.
+   (*mi_mappedblocks*)
+      intros. 
+      destruct (mkInjectionsN_4Val _ _ _ _ _ _ _ _ _ _ HeqMKI VBj23_1 _ _ _ H).
+           destruct H0. apply Fwd3. apply (VBj23_2 _ _ _  H0).
+           destruct H0 as [M [ZM [BM [J' B']]]].  eapply MInj13'. apply J'.
+   (*no_overlap*) intros b; intros.
+      destruct (mkInjectionsN_4Val _ _ _ _ _ _ _ _ _ _ HeqMKI VBj23_1 _ _ _ H0).
+         destruct H4 as [j23b vbb].
+         destruct (mkInjectionsN_4Val _ _ _ _ _ _ _ _ _ _ 
+               HeqMKI VBj23_1 _ _ _ H1).
+            destruct H4 as [j23b2 vbb2]. 
+            eapply MInj23. 
+               apply H. 
+               apply j23b. 
+               apply j23b2.
+               apply Fwd2. apply (VBj23_1 _ _ _ j23b). apply H2.
+               apply Fwd2. apply (VBj23_1 _ _ _ j23b2). apply H3.
+            destruct H4 as [M [ZM [BM [J' B']]]].
+            left. assert ( j23 b2 = None).
+                     remember (j23 b2) as d.
+                     destruct d; trivial.
+                     destruct p. apply eq_sym in Heqd.
+                     specialize (VBj23_1 _ _ _ Heqd). clear - VBj23_1 BM ZM.
+                     unfold Mem.valid_block in VBj23_1. exfalso. subst. omega.
+                  intros N; subst. 
+                  destruct (sep23 _ _ _ H4 H1). apply H6. 
+                  eapply MInj23. apply j23b.
+         destruct H4 as [M [ZM [NBb [j'b NBb']]]].
+           destruct (mkInjectionsN_4Val _ _ _ _ _ _ _ _ _ _ 
+                HeqMKI VBj23_1 _ _ _ H1).
+             destruct H4 as [j23b2 vbb2].  
+             left. assert ( j23 b = None).
+                      remember (j23 b) as d. 
+                      destruct d; trivial. destruct p.
+                      apply eq_sym in Heqd.
+                      specialize (VBj23_1 _ _ _ Heqd). clear - VBj23_1 NBb ZM.
+                      unfold Mem.valid_block in VBj23_1. exfalso. subst. omega.
+                   intros N; subst.
+                   destruct (sep23 _ _ _ H4 H0).
+                   apply H6. eapply MInj23. apply j23b2.
+      (*case where both blocks are in m2' but not in m2*)
+          destruct H4 as [M2 [ZM2 [NBb2 [j'b2 NBb2']]]]. subst.
+              assert (j23_None1: j23 (Mem.nextblock m2 + M) = None).
+                 remember (j23 (Mem.nextblock m2 + M)) as d. 
+                 destruct d; trivial. 
+                 apply eq_sym in Heqd. destruct p. 
+                 specialize (VBj23_1 _ _ _ Heqd). clear - VBj23_1 ZM.
+                 exfalso. unfold Mem.valid_block in VBj23_1.  omega.
+              assert (j23_None2: j23 (Mem.nextblock m2 + M2) = None).
+                 remember (j23 (Mem.nextblock m2 + M2)) as d. 
+                 destruct d; trivial. 
+                 apply eq_sym in Heqd. destruct p. 
+                 specialize (VBj23_1 _ _ _ Heqd). clear - VBj23_1 ZM2.
+                 exfalso. unfold Mem.valid_block in VBj23_1.  omega.      
+              destruct (sep23 _ _ _ j23_None1 H0) as [NV2_1 NV3_1].
+              destruct (sep23 _ _ _ j23_None2 H1) as [NV2_2 NV3_2].
+              assert (Max3_1:= Perm23' _ _ _ _ _ _ H0 H2).
+              assert (Max3_2:= Perm23' _ _ _ _ _ _ H1 H3).
+              assert (NEQ : Mem.nextblock m1 + M <> Mem.nextblock m1 + M2). 
+                 clear - H. intros N. apply H. 
+                 clear H. assert (M = M2). omega. 
+                          subst; trivial.
+              destruct (ACCESS  (Mem.nextblock m2 + M)) as [_ Invalid1].
+              specialize (Invalid1 NV2_1 Max ofs1).
+                           
+              remember (source (removeUndefs j12 j' prej12') 
+                    m1' (Mem.nextblock m2 + M) ofs1) as d.
+              destruct d.
+              (*source j12' ofs1 = Some*)
+                 destruct p. 
+                 rewrite (perm_subst _ _ _ _ _ _ _ Invalid1) in H2.
+                 clear Invalid1.
+                 destruct (ACCESS  (Mem.nextblock m2 + M2)) as [_ Invalid2].
+                 specialize (Invalid2 NV2_2 Max ofs2).
+
+                 remember (source (removeUndefs j12 j' prej12') m1'
+                         (Mem.nextblock m2 + M2) ofs2) as d.
+                 destruct d.
+                 (*source j12' ofs2 = Some*)
+                     destruct p. 
+                     rewrite (perm_subst _ _ _ _ _ _ _ Invalid2) in H3. 
+                     clear Invalid2.
+                     rename b into b1. rename z into z1. rename b0 into b2.
+                     rename z0 into z2. rename M into M1.
+
+                     destruct (source_SomeE _ _ _ _ _ Heqd) 
+                         as [bb1 [dd1 [ofs11 [PP [VB [ JJ' [PERM Off1]]]]]]].
+                     clear Heqd. subst. apply eq_sym in PP. inv PP.
+                     unfold removeUndefs in JJ'.
+                     remember (j12 b1) as q.
+                     destruct q; apply eq_sym in Heqq.
+                       destruct p. inv JJ'. exfalso. apply NV2_1. 
+                           apply (VBj12_2 _ _ _ Heqq).
+                     remember (j' b1) as qq.
+                     destruct qq; inv JJ'. apply eq_sym in Heqqq.
+                     destruct p. 
+                     destruct (mkInjectionsN_3V _ _ _ _ _ _ _ _ _ _ 
+                              HeqMKI VB12 VBj23_1 _ _ _ H5).
+                       destruct H4 as [? [? ?]]. clear -ZM H7. 
+                             exfalso. omega.
+                     destruct H4 as [MM1 [ZMM1 [BB1 [nbm [zz [X Y]]]]]]. 
+                     subst. apply Zplus_reg_l in nbm.
+                     apply eq_sym in nbm. subst. clear ZMM1 Y H2.
+                     destruct (source_SomeE _ _ _ _ _ Heqd0) as 
+                         [bb2 [dd2 [ofs22 [PP2 [VB2 [ JJ2' [PERM2 Off2]]]]]]].
+                     clear Heqd0. subst. apply eq_sym in PP2. inv PP2.
+                     unfold removeUndefs in JJ2'.
+                     remember (j12 b2) as r.
+                     destruct r; apply eq_sym in Heqr.
+                          destruct p. inv JJ2'. 
+                           exfalso. apply NV2_2. apply (VBj12_2 _ _ _ Heqr).
+                     remember (j' b2) as rr.
+                     destruct rr; inv JJ2'. apply eq_sym in Heqrr.
+                     destruct p. 
+                     destruct (mkInjectionsN_3V _ _ _ _ _ _ _ _
+                                         _ _ HeqMKI VB12 VBj23_1 _ _ _ H4).
+                       destruct H2 as [? [? ?]]. clear -ZM2 H7.
+                                          exfalso. omega.
+                     destruct H2 as [MM2 [ZMM2 [BB2 [nbm
+                                           [zz [X2 Y2]]]]]]. subst.
+                     apply Zplus_reg_l in nbm. apply eq_sym in nbm.  subst. 
+                     clear ZMM2 Y2 H3.
+
+                     eapply MInj13'. 
+                        apply NEQ. 
+                        assumption.
+                        assumption. 
+                        rewrite Zplus_0_r; trivial.
+                        rewrite Zplus_0_r; trivial.
+                 (*source j12' ofs2 = None*)
+                    unfold Mem.perm in H3. rewrite Invalid2 in H3. inv H3. 
+              (*source j12' ofs1 = Some*)
+                  unfold Mem.perm in H2. rewrite Invalid1 in H2. inv H2. 
+   (*mi_representable*) intros. rename b into b2.
+       destruct (mkInjectionsN_4Val _ _ _ _ _ _ _ _ _ _ HeqMKI VBj23_1 _ _ _ H).
+       (*first case*)
+         destruct H1 as [j23b2 Val2].
+         destruct (ACCESS b2) as [Valid _]. 
+         specialize (Valid Val2 k (Int.unsigned ofs)).
+         remember (source  j12 m1 b2 (Int.unsigned ofs)) as d.
+         destruct d. 
+         (*source  j12 m1 b2 (Int.unsigned ofs) = Some p0*)
+            destruct p0.
+            rewrite (perm_subst _ _ _ _ _ _ _ Valid) in H0. clear Valid.
+            destruct (source_SomeE _ _ _ _ _ Heqd) 
+                as [b1 [delta1 [ofs1 [PP [VB [ J12 [PERM Off1]]]]]]].
+            clear Heqd. subst. apply eq_sym in PP. inv PP.
+            assert (Val1 := Mem.perm_valid_block _ _ _ _ _ PERM).
+            rewrite <- (IP12 _ _ Max  PERM _ _ J12) in PERM.
+               eapply MInj23. apply j23b2. 
+            rewrite Off1. apply PERM.
+         (*source  j12 m1 b2 (Int.unsigned ofs) = None0*)
+            rewrite (perm_subst _ _ _ _ _ _ _ Valid) in H0. clear Valid.
+            eapply MInj23. apply j23b2. apply H0.
+       (*second case*)
+         destruct H1 as [M [ZM [B2 [J' X]]]]. subst.
+         destruct (ACCESS (Mem.nextblock m2 + M)) as [_ Invalid].
+         assert (Inval2: ~ Mem.valid_block m2 (Mem.nextblock m2 + M)).
+                clear - ZM. unfold Mem.valid_block. omega.
+         assert (MX: Mem.perm m2' (Mem.nextblock m2 + M) 
+                  (Int.unsigned ofs) Max Nonempty).
+                eapply Mem.perm_max. eapply Mem.perm_implies.
+                    apply H0. apply perm_any_N.
+         assert (InvMax:= Invalid Inval2 Max  (Int.unsigned ofs)).
+         specialize (Invalid Inval2 k (Int.unsigned ofs)).
+         remember (source (removeUndefs j12 j' prej12') m1'
+                        (Mem.nextblock m2 + M) (Int.unsigned ofs)) as d.
+         destruct d.
+         (*source (removeUndefs j12 j' prej12') ... = Some p0*) 
+             destruct p0.
+             rewrite (perm_subst _ _ _ _ _ _ _ Invalid) in *. clear Invalid.
+             rewrite (perm_subst _ _ _ _ _ _ _ InvMax) in *. clear InvMax.
+             destruct (source_SomeE _ _ _ _ _ Heqd) 
+                 as [b1 [delta1 [ofs1 [PP [VB [ J12 [PERM Off1]]]]]]].
+             clear Heqd. subst. apply eq_sym in PP. inv PP.
+             unfold removeUndefs in J12.
+             remember (j12 b) as r.
+             destruct r; apply eq_sym in Heqr.
+             (*case j12 = Some p0*)
+               destruct p0. inv J12. exfalso. 
+               apply Inval2. apply (VBj12_2 _ _ _ Heqr).
+             (*case j12 = None*)
+               remember (j' b) as rr.
+               destruct rr; inv J12. apply eq_sym in Heqrr.
+               destruct p0.  
+               destruct (mkInjectionsN_3V _ _ _ _ _ _ _ _ _ _ 
+                     HeqMKI VB12 VBj23_1 _ _ _ H2).
+               (*first case*)
+                  destruct H1 as [? [? ?]]. clear -ZM H4. exfalso. omega.
+               (*second case*)
+                  destruct H1 as [MM1 [ZMM1 [BB1 [nbm [zz [XX Y]]]]]]. subst. 
+                  rewrite Zplus_0_r in *. subst.
+                  apply Zplus_reg_l in nbm. apply eq_sym in nbm. subst.  
+                  clear ZMM1 Y.
+                  rewrite Heqrr in J'. inv J'.
+                  eapply (Mem.mi_representable _ _ _ MInj13'
+                             (Mem.nextblock m1 + M) ).
+                      apply Heqrr.
+                      apply H0.
+         (*source (removeUndefs j12 j' prej12') ... = None*) 
+            unfold Mem.perm in MX. rewrite InvMax in MX. inv MX.
+split. trivial.
+split; trivial.           
+split; trivial.           
+split; trivial.           
+split; trivial.           
+split; trivial.           
+split. intros.  
+  (*mem_wd m2'*)
+   apply mem_wdI. intros.
+   destruct (CONT b) as [ValidCONT InvalidCONT].
+   apply (valid_split _ _ _ _ (ACCESS b)); intros; clear ACCESS.
+   (*valid*)
+      clear InvalidCONT.
+      specialize (H1 Cur ofs). specialize (ValidCONT H0 ofs).
+      remember (source j12 m1 b ofs) as d.
+      destruct d. 
+      (*source  j12 m1 b ofs = Some p0*) 
+          destruct p. 
+          destruct (source_SomeE _ _ _ _ _ Heqd) 
+             as [bb1 [dd1 [ofs11 [PP [VB [ JJ [PERM Off2]]]]]]]. clear Heqd.
+          subst. apply eq_sym in PP. inv PP.
+          rewrite (perm_subst _ _ _ _ _ _ _ H1) in R. clear H1.
+          remember (j23' b) as q.
+          destruct q; apply eq_sym in Heqq.
+          (*j23' b = Some p*)
+             destruct p. rewrite ValidCONT. clear ValidCONT.
+             (*The following 19 lines are essentially repated below,
+               in the case INVALID - extract as ausiliary lemma?*)
+             remember (ZMap.get z (ZMap.get b0 (Mem.mem_contents m1'))) as v.
+             destruct v; simpl. constructor. constructor. unfold removeUndefs.
+             remember (j12 b2) as d.
+             destruct d; apply eq_sym in Heqd.
+                destruct p. econstructor. eapply flatinj_I.
+                    eapply Fwd2. apply (VBj12_2 _ _ _ Heqd).
+                    rewrite Int.add_zero. trivial.
+             remember (j' b2) as r.
+             destruct r; apply eq_sym in Heqr.
+                destruct p. rewrite IDextensional in Heqr. 
+                destruct (compose_meminjD_Some _ _ _ _ _ Heqr)
+                    as [bb1 [off1 [off [A [B C]]]]]. subst. clear Heqr.
+                 unfold removeUndefs in A.  
+                 rewrite Heqd in A.
+                 remember (j' b2) as u. 
+                 destruct u; inv A. 
+                   destruct p. rewrite H2.  econstructor. 
+                   eapply flatinj_I. eapply Mem.valid_block_inject_1. 
+                      apply B. apply Inj23'. rewrite Int.add_zero. trivial.
+                    constructor.
+          (*j23' b = None*) rewrite ValidCONT. clear ValidCONT.
+             assert (J23: j23 b = None). 
+                remember (j23 b) as dd.
+                destruct dd; apply eq_sym in Heqdd. 
+                   destruct p. rewrite (inc23 _ _ _ Heqdd) in Heqq.
+                                inv Heqq. trivial.
+                   eapply memval_inject_incr. apply mem_wd_E in WD2. 
+                 assert (MV:= Mem.mi_memval _ _ _ (Mem.mi_inj _ _ _ WD2)
+                           b (z+dd1)).
+                 rewrite flatinj_I in MV.
+                 specialize (MV _ _ (eq_refl _)).
+                 rewrite Zplus_0_r in MV. apply MV.
+                 rewrite (IP12 b0).
+                   destruct Unch11' as [Uperm _].
+                     rewrite Uperm. apply R. 
+                        unfold loc_unmapped, compose_meminj. rewrite JJ. 
+                           rewrite J23. trivial.
+                        apply (Mem.perm_valid_block _ _ _ _ _ PERM).
+                     apply PERM.
+                     apply JJ.
+                 apply H0.
+                 intros bb; intros. apply flatinj_E in H1. 
+                   destruct H1 as [? [? ?]]; subst. 
+                   apply flatinj_I. apply Fwd2. apply H3.
+      (*source  j12 m1 b ofs = None*) 
+          rewrite (perm_subst _ _ _ _ _ _ _ H1) in R. clear H1.
+          rewrite ValidCONT. clear ValidCONT.
+          assert (SRC:= source_NoneE _ _ _ _ Heqd). clear Heqd.
+          eapply memval_inject_incr. apply mem_wd_E in WD2. 
+            assert (MV:= Mem.mi_memval _ _ _ (Mem.mi_inj _ _ _ WD2) b ofs). 
+            rewrite flatinj_I in MV. 
+              specialize (MV _ _ (eq_refl _) R). 
+                 rewrite Zplus_0_r in MV. apply MV.
+              apply (Mem.perm_valid_block _ _ _ _ _ R).
+          intros bb; intros. apply flatinj_E in H1. 
+             destruct H1 as [? [? ?]]; subst. apply flatinj_I. 
+                 apply Fwd2. apply H3.
+   (*valid*)
+       clear ValidCONT.
+       specialize (H1 Cur ofs). specialize (InvalidCONT H0 ofs).
+       remember (source (removeUndefs j12 j' prej12') m1' b ofs) as d.
+       destruct d. 
+       (*source (removeUndefs j12 j' prej12') m1' b ofs  = Some p*)
+           destruct p. 
+           destruct (source_SomeE _ _ _ _ _ Heqd)
+               as [bb1 [dd1 [ofs11 [PP [VB [ JJ [PERM Off2]]]]]]]. clear Heqd.
+           subst. apply eq_sym in PP. inv PP.
+           rewrite (perm_subst _ _ _ _ _ _ _ H1) in R. clear H1.
+           rewrite InvalidCONT. clear InvalidCONT.
+            (*HERE's the repetition of those 19 lines, for b1 instead of b2*)
+             remember (ZMap.get z (ZMap.get b0 (Mem.mem_contents m1'))) as v.
+             destruct v; simpl. constructor. constructor. unfold removeUndefs.
+             remember (j12 b1) as d.
+             destruct d; apply eq_sym in Heqd.
+                destruct p. econstructor. eapply flatinj_I.
+                    eapply Fwd2. apply (VBj12_2 _ _ _ Heqd).
+                    rewrite Int.add_zero. trivial.
+             remember (j' b1) as r.
+             destruct r; apply eq_sym in Heqr.
+                destruct p. rewrite IDextensional in Heqr. 
+                destruct (compose_meminjD_Some _ _ _ _ _ Heqr)
+                    as [bb1 [off1 [off [A [B C]]]]]. subst. clear Heqr.
+                 unfold removeUndefs in A.  
+                 rewrite Heqd in A.
+                 remember (j' b1) as u. 
+                 destruct u; inv A. 
+                   destruct p. rewrite H2.  econstructor. 
+                   eapply flatinj_I. eapply Mem.valid_block_inject_1. 
+                      apply B. apply Inj23'. rewrite Int.add_zero. trivial.
+                    constructor.
+
+       (*source (removeUndefs j12 j' prej12') m1' b ofs = None*)
+            unfold Mem.perm in R. rewrite H1 in R. inv R.
+split; assumption.
+Qed.
+
+Parameter mkAccessMap_II_exists: forall (j12 j12':meminj) (m1 m1' m2: mem),
+                           ZMap.t (Z -> perm_kind -> option permission).
+Axiom mkAccessMap_II_ok: forall j12 j12' m1 m1' m2, 
+      AccessMap_II_Property j12 j12' m1 m1' m2 
+                   (mkAccessMap_II_exists  j12 j12' m1 m1' m2).
+
+Parameter mkContentsMap_II_exists: forall ( j12 j12' j23':meminj)
+             (m1 m1' m2:Mem.mem), ZMap.t (ZMap.t memval).
+Axiom mkContentsMap_II_ok: forall j12 j12' j23' m1 m1' m2, 
+      Content_II_Property  j12 j12' j23' m1 m1' m2
+                 (mkContentsMap_II_exists  j12 j12' j23' m1 m1' m2).
+
+Definition mkII m1 m2 j12 (MInj12 : Mem.inject j12 m1 m2) m1' 
+                   (Fwd1: mem_forward m1 m1') j23 m3
+                   (MInj23 : Mem.inject j23 m2 m3) m3'
+                   (Fwd3: mem_forward m3 m3')
+                   j' (MInj13': Mem.inject j' m1' m3')
+                   (InjIncr: inject_incr (compose_meminj j12 j23) j')
+                   (InjSep: inject_separated (compose_meminj j12 j23) j' m1 m3)
+                   (Unch11': my_mem_unchanged_on
+                             (loc_unmapped (compose_meminj j12 j23)) m1 m1')
+                   (Unch33': my_mem_unchanged_on 
+                        (loc_out_of_reach (compose_meminj j12 j23) m1) m3 m3')
+                   (WD1: mem_wd m1) (WD1': mem_wd m1') (WD2: mem_wd m2)
+                   (WD3: mem_wd m3) (WD3' : mem_wd m3')
+
+                   (IP12: inject_perm_nonempty j12 m1 m2) 
+                   (IP23: inject_perm_nonempty j23 m2 m3)
+                   (IPj': inject_perm_nonempty j' m1' m3')
+
+                   prej12' j23' n1' n2'
+                   (HeqMKI: mkInjections m1 m1' m2 j12 j23 j' = 
+                           (prej12', j23', n1', n2'))
+                   j12' (Hj12': j12'= removeUndefs j12 j' prej12')
+                   (AL12: inject_aligned j12) (AL23: inject_aligned j23)
+                   (AL13': inject_aligned j')
+                 : Mem.mem'.
+eapply Mem.mkmem with  (nextblock:=n2')
+                      (mem_access:=mkAccessMap_II_exists j12 j12' m1 m1' m2).
+  apply (mkContentsMap_II_exists  j12 j12' j23' m1 m1' m2).
+  destruct (mkInjectionsN_0 _ _ _ _ _ _ _ _ _ _ HeqMKI) as [_ A]; subst.
+         assert ( Mem.nextblock m2 > 0). apply m2.
+         omega.
+  (*access_max*)
+     intros. specialize (mkAccessMap_II_ok j12 j12' m1 m1' m2 b). intros.
+    apply (valid_split _ _ _ _ H); clear H; intros.
+    (*valid m2 b*) 
+           assert (CUR:= H0 Cur ofs).
+           specialize (H0 Max ofs).
+           remember (source j12 m1 b ofs) as d.
+           destruct d.
+               destruct p. rewrite H0. rewrite CUR. apply m1'.
+            rewrite H0. rewrite CUR. apply m2.
+    (*invalid m2 b*)
+           assert (CUR:= H0 Cur ofs).
+           specialize (H0 Max ofs).
+           remember (source j12' m1' b ofs) as d.
+           destruct d.
+               destruct p. rewrite H0. rewrite CUR. apply m1'.
+            rewrite H0. rewrite CUR. constructor.
+  (*nextblock_noaccess*)
+  assert (VBj12_1: forall (b1 b2 : block) (ofs2 : Z),
+               j12 b1 = Some (b2, ofs2) -> Mem.valid_block m1 b1).
+      intros. apply (Mem.valid_block_inject_1 _ _ _ _ _ _ H MInj12).
+  assert (VBj12_2: forall (b1 b2 : block) (ofs2 : Z),
+               j12 b1 = Some (b2, ofs2) -> Mem.valid_block m2 b2).
+      intros. apply (Mem.valid_block_inject_2 _ _ _ _ _ _ H MInj12).
+  assert (VBj23_1: forall (b1 b2 : block) (ofs2 : Z),
+               j23 b1 = Some (b2, ofs2) -> Mem.valid_block m2 b1).
+      intros. apply (Mem.valid_block_inject_1 _ _ _ _ _ _ H MInj23).
+  assert (VBj23_2: forall (b1 b2 : block) (ofs2 : Z),
+               j23 b1 = Some (b2, ofs2) -> Mem.valid_block m3 b2).
+      intros. apply (Mem.valid_block_inject_2 _ _ _ _ _ _ H MInj23).
+  assert (VB12: forall b3 b4 ofs3, j12 b3 = Some (b4, ofs3) -> 
+              b3 < Mem.nextblock m1 /\ b4 < Mem.nextblock m2).
+      intros. split. apply (VBj12_1 _ _ _ H). apply (VBj12_2 _ _ _ H).
+  intros. 
+  specialize (mkAccessMap_II_ok j12 j12' m1 m1' m2 b). intros AM.
+  apply (valid_split _ _ _ _ AM); clear AM; intros.
+  (*valid m2 b*) 
+      destruct (mkInjectionsN_0 _ _ _ _ _ _ _ _ _ _ HeqMKI) as [_ A]; subst. 
+      unfold Mem.valid_block in H0.
+      exfalso. clear - H H0. omega.
+  (*invalid m2 b*)
+      specialize (H1 k ofs).
+      remember (source j12' m1' b ofs) as d.
+      destruct d.
+         destruct p. rewrite H1. clear H1. 
+         destruct (source_SomeE _ _ _ _ _ Heqd)
+             as [bb1 [dd1 [ofs11 [PP [VB [ JJ [PERM Off2]]]]]]]. clear Heqd.
+         subst. apply eq_sym in PP. inv PP.
+         exfalso. unfold removeUndefs in JJ.
+         remember (j12 b0) as d.
+         destruct d. 
+             destruct p. inv JJ. apply eq_sym in Heqd. 
+             apply H0. eapply Mem.valid_block_inject_2.
+                     apply Heqd. apply MInj12.
+         remember (j' b0) as d.
+         destruct d.
+           destruct p.
+           destruct (mkInjectionsN_3V _ _ _ _ _ _ _ _ _ _
+                 HeqMKI VB12 VBj23_1 _ _ _ JJ).
+               destruct H1 as [? [? ?]]. apply H0. apply (VBj12_2 _ _ _ H1).
+               destruct H1 as [M [ZM [B0 [B2 [D [A B]]]]]]. subst. 
+                  clear - H B. omega.
+         inv JJ.
+      apply H1.
+Defined.
+
+Lemma my_interpolate_II: forall m1 m2 j12 (MInj12 : Mem.inject j12 m1 m2) m1'
+              (Fwd1: mem_forward m1 m1') j23 m3
+              (MInj23 : Mem.inject j23 m2 m3) m3' (Fwd3: mem_forward m3 m3')
+              j' (MInj13': Mem.inject j' m1' m3')
+              (InjIncr: inject_incr (compose_meminj j12 j23) j')
+              (InjSep: inject_separated (compose_meminj j12 j23) j' m1 m3)
+              (Unch11': my_mem_unchanged_on
+                          (loc_unmapped (compose_meminj j12 j23)) m1 m1')
+              (Unch33': my_mem_unchanged_on
+                     (loc_out_of_reach (compose_meminj j12 j23) m1) m3 m3')
+              (WD1: mem_wd m1) (WD1': mem_wd m1') (WD2: mem_wd m2)
+              (WD3: mem_wd m3) (WD3' : mem_wd m3'),
+         exists m2', exists j12', exists j23', 
+                j'=compose_meminj j12' j23' /\
+                inject_incr j12 j12' /\ inject_incr j23 j23' /\
+                Mem.inject j12' m1' m2' /\ mem_forward m2 m2' /\
+                Mem.inject j23' m2' m3' /\
+                my_mem_unchanged_on (loc_out_of_reach j12 m1) m2 m2' /\
+                inject_separated j12 j12' m1 m2 /\
+                inject_separated j23 j23' m2 m3 /\
+                my_mem_unchanged_on (loc_unmapped j23) m2 m2' /\ 
+                my_mem_unchanged_on (loc_out_of_reach j23 m2) m3 m3' /\
+                (mem_wd m2 -> mem_wd m2').                             
+Proof. intros.
+  remember (mkInjections m1 m1' m2 j12 j23 j') as MKI.
+  apply eq_sym in HeqMKI. destruct MKI as [[[j12' j23'] n1'] n2'].
+  assert (VBj12_1: forall (b1 b2 : block) (ofs2 : Z),
+                j12 b1 = Some (b2, ofs2) -> Mem.valid_block m1 b1).
+      intros. apply (Mem.valid_block_inject_1 _ _ _ _ _ _ H MInj12).
+  assert (VBj12_2: forall (b1 b2 : block) (ofs2 : Z),
+                j12 b1 = Some (b2, ofs2) -> Mem.valid_block m2 b2).
+      intros. apply (Mem.valid_block_inject_2 _ _ _ _ _ _ H MInj12).
+  assert (VBj23: forall (b1 b2 : block) (ofs2 : Z),
+                j23 b1 = Some (b2, ofs2) -> Mem.valid_block m2 b1).
+      intros. apply (Mem.valid_block_inject_1 _ _ _ _ _ _ H MInj23).
+  assert (inc12:= mkInjections_1_injinc _ _ _ _ _ _ _ _ _ _ HeqMKI VBj12_1).
+  assert (sep12:= mkInjections_1_injsep _ _ _ _ _ _ _ _ _ _ HeqMKI).
+  assert (inc23:= mkInjections_2_injinc _ _ _ _ _ _ _ _ _ _ HeqMKI VBj23).
+  assert (sep23:= mkInjections_2_injsep _ _ _ _ _ _ _ _ _ _ 
+                   HeqMKI VBj12_1 _ InjSep).
+  assert (NB1: Mem.nextblock m1' - Mem.nextblock m1 >= 0).
+     assert (B: forall b, b <= Mem.nextblock m1 -> b <= Mem.nextblock m1'). 
+         intros. destruct (Fwd1 (b -1)).  unfold Mem.valid_block. omega. 
+                   unfold Mem.valid_block in H0. omega. 
+     clear -B. specialize (B (Mem.nextblock m1)). omega. 
+  destruct (mkInjectionsN_0  _ _ _ _ _ _ _ _ _ _ HeqMKI) as [N1 _].
+       rewrite (nat_of_Z_eq _ NB1) in N1. 
+       rewrite Zplus_minus in N1. subst.
+  assert (VBj': forall b1 b3 ofs3, j' b1 = Some (b3, ofs3) ->
+             b1 < Mem.nextblock m1').
+      intros. apply (Mem.valid_block_inject_1 _ _ _ _ _ _ H MInj13').
+  assert (ID:= RU_composememinj _ _ _ _ _ _ _ _ _ _ HeqMKI InjIncr _ 
+                 InjSep VBj12_1 VBj12_2 VBj23 VBj').
+  assert (IP12:= inj_implies_inject_perm_nonenempty _ _ _  MInj12).
+  assert (IP23:= inj_implies_inject_perm_nonenempty _ _ _  MInj23).
+  assert (IP13':= inj_implies_inject_perm_nonenempty _ _ _  MInj13').
+  assert (AL12:= inj_implies_inject_aligned _ _ _  MInj12). 
+  assert (AL23:= inj_implies_inject_aligned _ _ _  MInj23). 
+  assert (AL13':= inj_implies_inject_aligned _ _ _  MInj13').
+  assert (XX: Mem.nextblock  
+                    (mkII m1 m2 j12 MInj12 m1' Fwd1 j23 m3
+                             MInj23 m3' Fwd3
+                             j' MInj13'
+                             InjIncr
+                             InjSep
+                             Unch11'
+                             Unch33'
+                             WD1 WD1' WD2 WD3 WD3' IP12 IP23  IP13' _ _ _ _
+                             HeqMKI _ (eq_refl _) AL12 AL23 AL13') 
+                  = n2').
+           reflexivity.
+   assert (YY:Content_II_Property j12 (removeUndefs j12 j' j12') j23' m1 m1' m2
+                  (Mem.mem_contents
+                       (mkII m1 m2 j12 MInj12 m1' Fwd1 j23 m3
+                             MInj23 m3' Fwd3
+                             j' MInj13'
+                             InjIncr
+                             InjSep
+                             Unch11'
+                             Unch33'
+                             WD1 WD1' WD2 WD3 WD3' IP12 IP23  IP13' _ _ _ _ 
+                             HeqMKI _ (eq_refl _) AL12 AL23 AL13') )).
+                     simpl. apply mkContentsMap_II_ok.
+  assert (ZZ: AccessMap_II_Property j12 (removeUndefs j12 j' j12') m1 m1' m2
+                  (Mem.mem_access
+                       (mkII m1 m2 j12 MInj12 m1' Fwd1 j23 m3
+                             MInj23 m3' Fwd3
+                             j' MInj13'
+                             InjIncr
+                             InjSep
+                             Unch11'
+                             Unch33'
+                             WD1 WD1' WD2 WD3 WD3' IP12 IP23  IP13' _ _ _ _ 
+                             HeqMKI _ (eq_refl _) AL12 AL23 AL13') )).
+                     simpl. apply mkAccessMap_II_ok.
+  destruct (II_ok m1 m2 j12 MInj12 m1' Fwd1 j23 m3
+                             MInj23 m3' Fwd3
+                             j' MInj13'
+                             InjIncr
+                             InjSep
+                             Unch11'
+                             Unch33'
+                             WD1 WD1' WD2 WD3 WD3' IP12 IP23 IP13' _ _ _ _ 
+                             HeqMKI _ (eq_refl _) _ XX YY ZZ AL12 AL23 AL13')
+       as [A [B [C [D [E [F [G [H [I [J [K [L [M [N [O P]]]]]]]]]]]]]]].
+  eexists.  exists (removeUndefs j12 j' j12') . exists j23'.
+  split; trivial.
+  split; trivial.
+  split; trivial.
+  split. eassumption. auto.
+  split; trivial.
+  split; trivial.
+  split; trivial.
+  split; trivial.
+  split; trivial.
+  split; trivial.
+  split; trivial.
+Qed.
+
+Lemma interpolate_II: forall m1 m2 j12 (MInj12 : Mem.inject j12 m1 m2) m1'
+                  (Fwd1: mem_forward m1 m1') j23 m3
+                  (MInj23 : Mem.inject j23 m2 m3) m3' (Fwd3: mem_forward m3 m3')
+                  j' (MInj13': Mem.inject j' m1' m3')
+                  (InjIncr: inject_incr (compose_meminj j12 j23) j')
+                  (InjSep: inject_separated (compose_meminj j12 j23) j' m1 m3)
+                  (Unch11': mem_unchanged_on 
+                            (loc_unmapped (compose_meminj j12 j23)) m1 m1')
+                  (Unch33': mem_unchanged_on
+                        (loc_out_of_reach (compose_meminj j12 j23) m1) m3 m3')
+                  (WD1: mem_wd m1) (WD1': mem_wd m1') (WD2: mem_wd m2)
+                  (WD3: mem_wd m3) (WD3' : mem_wd m3'),
+         exists m2', exists j12', exists j23', j'=compose_meminj j12' j23' /\
+                   inject_incr j12 j12' /\ inject_incr j23 j23' /\
+                   Mem.inject j12' m1' m2' /\ mem_forward m2 m2' /\ 
+                   Mem.inject j23' m2' m3' /\
+                   mem_unchanged_on (loc_out_of_reach j12 m1) m2 m2' /\
+                   inject_separated j12 j12' m1 m2 /\ 
+                   inject_separated j23 j23' m2 m3 /\
+                   mem_unchanged_on (loc_unmapped j23) m2 m2' /\ 
+                   mem_unchanged_on (loc_out_of_reach j23 m2) m3 m3' /\
+                   (mem_wd m2 -> mem_wd m2').                             
+Proof. intros.
+  rewrite <- unchAx in Unch11', Unch33'.
+  destruct (my_interpolate_II m1 m2 j12 MInj12 m1' Fwd1 j23 m3
+                             MInj23 m3' Fwd3
+                             j' MInj13'
+                             InjIncr
+                             InjSep
+                             Unch11'
+                             Unch33'
+                             WD1 WD1' WD2 WD3 WD3') 
+       as [m2' [j12' [j23' [A [B [C [D [E [F [G [H [I [J [K L]]]]]]]]]]]]]].
+  exists m2'. exists j12'. exists j23'.
+  rewrite unchAx in G, J, K. repeat (split; trivial).
+Qed.
