compositional_compcert/mem_interpolation_proofs.v
@@ -1,0 +1,14 @@
+Load loadpath.
+Require Import compositional_compcert.mem_interpolants.
+Require Import compositional_compcert.mem_interpolation_EE.
+Require Import compositional_compcert.mem_interpolation_EI.
+Require Import compositional_compcert.mem_interpolation_IE.
+Require Import compositional_compcert.mem_interpolation_II.
+
+Module MemoryInterpolations <: MemoryInterpolationAxioms.
+Definition  interpolate_II := interpolate_II.
+Definition  interpolate_EI := interpolate_EI.
+Definition  interpolate_IE := interpolate_IE.
+Definition  interpolate_EE := interpolate_EE.
+End MemoryInterpolations.
+
